stmt and e test

hol/stmt_test.sml
@@ -9,6 +9,11 @@ open wordsTheory;
 open optionTheory;
 open sumTheory;
 
+
+val STMT_SIMP = RW.ONCE_RW_TAC[stmt_red_cases] >> EVAL_TAC>> FULL_SIMP_TAC std_ss [];
+val EXP_SIMP = RW.ONCE_RW_TAC[e_red_cases] >> EVAL_TAC>> FULL_SIMP_TAC std_ss [];
+
+
 (* bits representations*)
 val bitE    = ``v_bit ([] ,0)``;
 val bitT    = ``v_bit ([T],1)``;
@@ -25,29 +30,31 @@ val Parse_Rej = ``(status_pars_next (pars_next_pars_fin pars_finreject))``;
 val Parse_Acc = ``(status_pars_next (pars_next_pars_fin pars_finaccept))``;
 
 
-(*mappings from one variable to a tuple (value, string option)*)
-val map0  = ``("x", (^bitE , NONE: string option))``;
-val map1  = ``("x", (^bitT , NONE: string option))``;
-val map2  = ``("x", (^bitF , NONE: string option))``;
-val map3  = ``("y", (^bitE , NONE: string option))``;
-val map4  = ``("y", (^bitT , NONE: string option))``;
-val map5  = ``("y", (^bitF , NONE: string option))``;
-val map6  = ``("z", (^bitE , NONE: string option))``;
-val map7  = ``("z", (^bitT , NONE: string option))``;
-val map8  = ``("z", (^bitF , NONE: string option))``;
-val map9  = ``("x", (^bitA , NONE: string option))``;
-val map10 = ``("x", (^bitA , NONE: string option))``;
-val map11 = ``("parseError", (^bitErr1 , NONE: string option))``;
-val map12 = ``("parseError", (^bitErr2 , NONE: string option))``;
-val map13  = ``("y", (^bitF , SOME "x"))``;
-val map14 = ``("headers.ip.ttl", (^bitTwo, NONE:string option)) ``;
-val map15  = ``("a", (^bitF , NONE: string option))``;
-val map16  = ``("b", (^bitF , SOME "y"))``;
-val map17 = ``("headers.ip.ttl", (^bitF, NONE:string option)) ``;
-
+(*mappings from one variable to a tuple (value, lval option)*)
+val map0  = ``(varn_name "x", (^bitE , NONE: lval option))``;
+val map1  = ``(varn_name "x", (^bitT , NONE: lval option))``;
+val map2  = ``(varn_name "x", (^bitF , NONE: lval option))``;
+val map3  = ``(varn_name "y", (^bitE , NONE: lval option))``;
+val map4  = ``(varn_name "y", (^bitT , NONE: lval option))``;
+val map5  = ``(varn_name "y", (^bitF , NONE: lval option))``;
+val map6  = ``(varn_name "z", (^bitE , NONE: lval option))``;
+val map7  = ``(varn_name "z", (^bitT , NONE: lval option))``;
+val map8  = ``(varn_name "z", (^bitF , NONE: lval option))``;
+val map9  = ``(varn_name "x", (^bitA , NONE: lval option))``;
+val map10 = ``(varn_name "x", (^bitA , NONE: lval option))``;
+val map11 = ``(varn_name "parseError", (^bitErr1 , NONE: lval option))``;
+val map12 = ``(varn_name "parseError", (^bitErr2 , NONE: lval option))``;
+val map13 = ``(varn_name "y",         (^bitF    , SOME (lval_varname (varn_name"x"))))``;
+val map14 = ``(varn_name "headers.ip.ttl", (^bitTwo, NONE:lval option)) ``;
+val map15 = ``(varn_name "a", (^bitF , NONE: lval option))``;
+val map16 = ``(varn_name "b", (^bitF , SOME (lval_varname (varn_name"y"))))``;
+val map17 = ``(varn_name "headers.ip.ttl", (^bitF, NONE:lval option)) ``;
+val map18 = ``(varn_star,  ((v_bit ([F; F],2)),NONE:lval option) )``; 
+val map19 = ``(varn_star,  (v_bit (ARB),NONE:lval option) )``;
+val map20 = ``(varn_star,  ((v_bit ([F; F],2)),NONE:lval option) )``;
 
 (*scopes examples*)
-val scope0 = ``(FEMPTY |+ ^map0)``;
+val scope0 = ``(FEMPTY |+ ^map0): scope``;
 val scope1 = ``(FEMPTY |+ ^map1)``;
 val scope2 = ``(FEMPTY |+ ^map2)``;
 val scope3 = ``(FEMPTY |+ ^map1 |+ ^map4)``;
@@ -61,10 +68,16 @@ val scope10 = ``(FEMPTY |+ ^map7 |+ ^map12)``;
 val scope11 = ``(FEMPTY |+ ^map4 |+ ^map2)``;
 val scope13 = ``(FEMPTY |+ ^map5)``;
 val scope14 = ``(FEMPTY |+ ^map13)``;
-val scope15 = ``(FEMPTY |+ ^map15 |+ ^map16)``; 
+val scope15 = ``(FEMPTY |+ ^map15 |+ ^map16)``;
 val scope16 = ``(FEMPTY |+ ^map14)``;
-val scope17 = ``(FEMPTY |+ ^map15)``;
+val scope17 = ``(FEMPTY |+ ^map15):scope``;
 val scope18 = ``(FEMPTY |+ ^map17)``;
+val scope19 = ``(FEMPTY |+ ^map4 |+ ^map2 |+ ^map18)``;
+val scope20 = ``(FEMPTY |+ ^map4 |+ ^map2)``;
+val scope21 = ``(FEMPTY |+ ^map1 |+ ^map4|+ ^map9)``;
+val scope22 = ``(FEMPTY |+ ^map4 |+ ^map2 |+ ^map19):scope``;
+val scope23 = ``(FEMPTY |+ ^map20):scope``;
+
 
 (*scope list examples*)
 val scopelist0 = ``[^scope0]``;
@@ -93,6 +106,11 @@ val scopelist22 = ``[^scope16]``;
 val scopelist23 = ``[^scope8; ^scope17]``;
 val scopelist24 = ``[^scope18]``;
 val scopelist25 = ``[^scope11; ^scope14]``;
+val scopelist26 = ``[^scope14]``;
+val scopelist27 = ``[^scope19]``;
+val scopelist28 = ``[^scope20]``;
+val scopelist29 = ``[^scope22]``;
+val scopelist30 = ``[^scope23]``;
 
 (*empty ctrl*)
 val empty_ctrl =
@@ -105,304 +123,276 @@ val ctx_empty = ``(FEMPTY, FEMPTY, FEMPTY, FEMPTY, empty_ctrl):ctx``;
 
 
 (*** assignment statement reduction --concrete values -- ***)
-val state1  = ``(state_tup (stacks_tup ^scopelist1 []) ^R): state``;
-val state2  = ``(state_tup (stacks_tup ^scopelist2 []) ^R): state``;
-val state2b = ``(state_tup (stacks_tup ^scopelist6 []) ^R): state``;
-val state2c = ``(state_tup (stacks_tup ^scopelist17 []) ^R): state``;
-val state2d = ``(state_tup (stacks_tup ^scopelist4 []) ^R): state``;
 
-val prog1  = ``(stmt_ass (lval_varname "x") (e_v (v_bit ([T], 1))))``;
-val prog2  = ``(stmt_ass (lval_varname "x") (e_v (v_bit ([F], 1))))``;
-val exp1   = ``(e_binop (e_v (v_bit ([T],1))) binop_add (e_v (v_bit ([F],1))))``;
-val prog2c = ``(stmt_ass (lval_varname "x") (^exp1) )``; (*assign with reduction*)
-val prog2d = ``(stmt_ass (lval_varname "x") (e_v (v_bit ([T],1))) )``; 
-val prog2e = ``(stmt_ass (lval_varname "x") (e_var("y") ))``;
+(* test 1: Pre/post frames and states for assignment with empty global*)
+val prog_ass1  = ``(stmt_ass (lval_varname (varn_name "x")) (e_v (v_bit ([T], 1))))``;
+val frame1a = `` [("f", ^prog_ass1 , ^scopelist1 )] : Frame_list `` ;
+val state1a = `` (state_P4 FEMPTY  ^frame1a ^R)  : state `` ;
+val frame1b = `` [("f", stmt_empty , ^scopelist2 )] : Frame_list `` ;
+val state1b = `` (state_P4 FEMPTY  ^frame1b ^R)  : state `` ;
+
 
 val test_stmt_ass1 =
-prove(`` stmt_red ^ctx_empty (^prog1) 
-                  (^state1)
-                  stmt_empty
-                  (^state2)  ``,
-RW.ONCE_RW_TAC[e_red_cases] >>
+prove(`` stmt_red ^ctx_empty ^state1a ^state1b ``,
+STMT_SIMP >>
 EVAL_TAC>>
-FULL_SIMP_TAC std_ss []>>
-EVAL_TAC>>
-SIMP_TAC std_ss [FUPDATE_EQ]
+SIMP_TAC std_ss [FUPDATE_EQ]>>
+FULL_SIMP_TAC list_ss []
 );
+
+
+
+(* test 2: Pre/post frames and states for assignment with non empty global*)
+val frame2a = `` [("f", ^prog_ass1 , ^scopelist1 )] : Frame_list `` ;
+val state2a = `` (state_P4 ^scope0  ^frame2a ^R)  : state `` ;
+val frame2b = `` [("f", stmt_empty , ^scopelist2 )] : Frame_list `` ;
+val state2b = `` (state_P4 ^scope0   ^frame2b ^R)  : state `` ;
 
 
 val test_stmt_ass2 =
-prove(`` stmt_red (^ctx_empty) (^prog2) 
-                  (^state2)
-                  stmt_empty
-                  (^state1)  ``,
-RW.ONCE_RW_TAC[e_red_cases] >>
+prove(`` stmt_red ^ctx_empty ^state2a ^state2b ``,
+STMT_SIMP >>
 EVAL_TAC>>
-FULL_SIMP_TAC std_ss []>>
-EVAL_TAC>>
-SIMP_TAC std_ss [FUPDATE_EQ]
+SIMP_TAC std_ss [FUPDATE_EQ]>>
+FULL_SIMP_TAC list_ss []
 );
+
+
+
+(* test 3: Pre/post frames and states for assignment with expression reduction*)
+val exp1   = ``(e_binop (e_v (v_bit ([T],1))) binop_add (e_v (v_bit ([F],1))))``;
+val prog_ass2 = ``(stmt_ass (lval_varname (varn_name "x")) (^exp1) )``;
+val prog_ass3 = ``(stmt_ass (lval_varname (varn_name "x")) (e_v (v_bit ([T],1))) )``; 
+val frame3a = `` [("f", ^prog_ass2 , ^scopelist1 )] : Frame_list `` ;
+val state3a = `` (state_P4 ^scope0  ^frame3a ^R)  : state `` ;
+val frame3b = `` [("f", ^prog_ass3 , ^scopelist1 )] : Frame_list `` ;
+val state3b = `` (state_P4 ^scope0   ^frame3b ^R)  : state `` ;
 
 
 val test_stmt_ass3 =
-prove(`` stmt_red (^ctx_empty) (^prog2) 
-                  (^state2b)
-                  stmt_empty
-                  (^state1)  ``,
-RW.ONCE_RW_TAC[e_red_cases] >>
-EVAL_TAC>>
-FULL_SIMP_TAC std_ss []>>
-EVAL_TAC>>
-SIMP_TAC std_ss [FUPDATE_EQ]
+prove(`` stmt_red ^ctx_empty ^state3a ^state3b ``,
+STMT_SIMP >>
+REPEAT (EXP_SIMP)
 );
 
 
+
+(* test 4: Pre/post frames and states for assignment with an other value*)
+val prog_ass4 = ``(stmt_ass (lval_varname (varn_name "x")) (e_var(varn_name "y")))``;
+val prog_ass5 = ``(stmt_ass (lval_varname (varn_name "x")) (e_v (v_bit ([T],1))) )``;
+val frame4a = `` [("f", ^prog_ass4 , ^scopelist17 )] : Frame_list `` ;
+val state4a = `` (state_P4 ^scope0  ^frame4a ^R)  : state `` ;
+val frame4b = `` [("f", ^prog_ass5 , ^scopelist17 )] : Frame_list `` ;
+val state4b = `` (state_P4 ^scope0  ^frame4b ^R)  : state `` ;
 
 val test_stmt_ass4 =
-prove(`` stmt_red (^ctx_empty) (^prog2c) 
-                  (^state1)
-                  (^prog2d)
-                  (^state1)  ``,
-REPEAT(RW.ONCE_RW_TAC[e_red_cases] >>
-EVAL_TAC>>
-FULL_SIMP_TAC std_ss [])
+prove(`` stmt_red ^ctx_empty ^state4a ^state4b ``,
+STMT_SIMP >>
+REPEAT (EXP_SIMP)
 );
 
 
-val test_stmt_ass5 =
-prove(`` stmt_red (^ctx_empty) (^prog2e) 
-                  (^state2c)
-                  (^prog2d)
-                  (^state2c)  ``,
-REPEAT(RW.ONCE_RW_TAC[e_red_cases] >>
-EVAL_TAC>>
-FULL_SIMP_TAC std_ss [])
-);
 
 
-val test_stmt_ass6 =
-prove(`` stmt_red ^ctx_empty (^prog1) 
-                  (^state2)
-                  stmt_empty
-                  (^state2)  ``,
-RW.ONCE_RW_TAC[e_red_cases] >>
-EVAL_TAC>>
-FULL_SIMP_TAC std_ss []>>
-EVAL_TAC>>
-SIMP_TAC std_ss [FUPDATE_EQ]
-);
 
-
-(*** if statement reduction --concrete values --  ***)
-val prog3a = ``(stmt_cond (e_v (v_bool  T )) stmt_empty  ^prog2 )``;
-val prog4a = ``(stmt_cond (e_v (v_bool  F )) stmt_empty  ^prog2 )``;
+(*** if statement reduction  ***)
 val cond1  = ``(e_binop (e_v (v_bit ([F],1))) binop_eq (e_v (v_bit ([F],1))))``;
 val cond2  = ``(e_binop (e_v (v_bit ([F],1))) binop_eq (e_v (v_bit ([T],1))))``;
-val prog3b = ``(stmt_cond  ^cond1 stmt_empty  ^prog2 )``;
-val prog4b = ``(stmt_cond  ^cond2 stmt_empty  ^prog2 )``;
+val prog_if1 = ``(stmt_cond  ^cond1 stmt_empty  ^prog_ass1 )``;
+val prog_if2 = ``(stmt_cond  ^cond2 stmt_empty  ^prog_ass1 )``;
+val prog_if3 = ``(stmt_cond (e_v (v_bool  T )) stmt_empty  ^prog_ass1 )``;
+val prog_if4 = ``(stmt_cond (e_v (v_bool  F )) stmt_empty  ^prog_ass1 )``;
 
+
+val frame_if1 = `` [("f", ^prog_if1 , ^scopelist1 )] : Frame_list `` ;
+val state_if1 = `` (state_P4 ^scope0  ^frame_if1 ^R)  : state `` ;
+
+val frame_if2 = `` [("f", ^prog_if3 , ^scopelist1 )] : Frame_list `` ;
+val state_if2 = `` (state_P4 ^scope0  ^frame_if2 ^R)  : state `` ;
+
+val frame_if3 = `` [("f", stmt_empty , ^scopelist1 )] : Frame_list `` ;
+val state_if3 = `` (state_P4 ^scope0  ^frame_if3 ^R)  : state `` ;
+
+val frame_if4 = `` [("f", ^prog_if2 , ^scopelist1 )] : Frame_list `` ;
+val state_if4 = `` (state_P4 ^scope0  ^frame_if4 ^R)  : state `` ;
+
+val frame_if5 = `` [("f", ^prog_if4 , ^scopelist1 )] : Frame_list `` ;
+val state_if5 = `` (state_P4 ^scope0  ^frame_if5 ^R)  : state `` ;
+
+
+(* test 1: tranistion for if e *)
 val test_stmt_cond1 =
-prove(`` stmt_red (^ctx_empty) (^prog3a) 
-                  (^state1)
-                  stmt_empty
-                  (^state1)  ``,
-RW.ONCE_RW_TAC[e_red_cases] >>
-EVAL_TAC>>
-FULL_SIMP_TAC std_ss []
+prove(`` stmt_red ^ctx_empty ^state_if1 ^state_if2  ``,
+STMT_SIMP >>
+REPEAT (EXP_SIMP)
 );
 
-
+(* test 2: transition for if true*)
 val test_stmt_cond2 =
-prove(`` stmt_red (^ctx_empty) (^prog4a) 
-                  (^state1)
-                  (^prog2)
-                  (^state1)  ``,
-RW.ONCE_RW_TAC[e_red_cases] >>
-EVAL_TAC>>
-FULL_SIMP_TAC std_ss []
+prove(`` stmt_red ^ctx_empty ^state_if2 ^state_if3  ``,
+STMT_SIMP >>
+REPEAT (EXP_SIMP)
 );
 
-
+(* test 3: transition for if e -> if false*)
 val test_stmt_cond3 =
-prove(`` stmt_red (^ctx_empty) (^prog3b) 
-                  (^state1)
-                  (^prog3a)
-                  (^state1)  ``,
-REPEAT (RW.ONCE_RW_TAC[e_red_cases] >>
-EVAL_TAC>>
-FULL_SIMP_TAC std_ss [])
-);
-
-val test_stmt_cond4 =
-prove(`` stmt_red (^ctx_empty) (^prog4b) 
-                  (^state1)
-                  (^prog4a)
-                  (^state1)  ``,
-REPEAT (RW.ONCE_RW_TAC[e_red_cases] >>
-EVAL_TAC>>
-FULL_SIMP_TAC std_ss [])
+prove(`` stmt_red ^ctx_empty ^state_if4 ^state_if5  ``,
+STMT_SIMP >>
+REPEAT (EXP_SIMP)
 );
 
 
 
+(*** declare statement reduction ***)
 
-(*** declare statement reduction --concrete values -- ***)
-val state3 = ``(state_tup (stacks_tup ^scopelist5 []) ^R): state``;
-val state4 = ``(state_tup (stacks_tup ^scopelist6 []) ^R): state``;
-val prog5  = ``(stmt_declare "x"  (t_base bt_bit) )``;
+(*declare a variable*)
+val prog_dec1  = ``(stmt_declare "x"  (t_base bt_bit) )``;
 
+val frame_dec1 = `` [("f", ^prog_dec1 , ^scopelist5 )] : Frame_list `` ;
+val state_dec1 = `` (state_P4 FEMPTY  ^frame_dec1 ^R)  : state `` ;
+
+val frame_dec2 = `` [("f", stmt_empty , ^scopelist6 )] : Frame_list `` ;
+val state_dec2 = ``(state_P4 FEMPTY  ^frame_dec2 ^R): state``;
+
+(* test 1: transition for declare with empty global*)
 val test_stmt_decl1 =
-prove(`` stmt_red (^ctx_empty) (^prog5) 
-                  (^state3)
-                  stmt_empty
-                  (^state4)  ``,
-RW.ONCE_RW_TAC[e_red_cases] >>
-EVAL_TAC>>
+prove(`` stmt_red (^ctx_empty) ^state_dec1 ^state_dec2  ``,
+STMT_SIMP >>
 FULL_SIMP_TAC list_ss [LUPDATE_def, arb_from_t_def]  
 );
 
 
+val frame_dec3 = `` [("f", ^prog_dec1 , ^scopelist5 )] : Frame_list `` ;
+val state_dec3 = `` (state_P4 ^scope5  ^frame_dec1 ^R)  : state `` ;
 
+val frame_dec4 = `` [("f", stmt_empty , ^scopelist6 )] : Frame_list `` ;
+val state_dec4 = ``(state_P4 ^scope5  ^frame_dec2 ^R): state``;
 
-val state5 = ``(state_tup (stacks_tup ^scopelist10 []) ^R): state``;
-val state6 = ``(state_tup (stacks_tup ^scopelist13 []) ^R): state``;
-
+(* test 2: transition for declare with non empty global*)
 val test_stmt_decl2 =
-prove(`` stmt_red (^ctx_empty) (^prog5) 
-                  (^state5)
-                  stmt_empty
-                  (^state6)  ``,
-RW.ONCE_RW_TAC[e_red_cases] >>
-EVAL_TAC>>
-FULL_SIMP_TAC list_ss [LUPDATE_def, arb_from_t_def]  
+prove(`` stmt_red (^ctx_empty) ^state_dec3 ^state_dec4  ``,
+STMT_SIMP >>
+EVAL_TAC
 );
+
 
 
 (*** block enter, exec, exit statement reduction --concrete values -- ***)
-val state7 = ``(state_tup (stacks_tup ^scopelist10 []) ^R): state``;
-val state8 = ``(state_tup (stacks_tup ^scopelist11 []) ^R): state``;
-val state9 = ``(state_tup (stacks_tup ^scopelist12 []) ^R): state``;
-val prog6a =  ``(stmt_block ^prog5 )``;
-val prog6b =  ``(stmt_block_ip ^prog5)``;
-val prog6c =  ``(stmt_block_ip stmt_empty)``;
+val prog_blk1 =  ``(stmt_block ^prog_if3 )``;
+val prog_blk2 =  ``(stmt_block_ip ^prog_if3)``;
+val prog_blk3 =  ``(stmt_block_ip stmt_empty)``;
+
+
+val frame_blk1 = `` [("f", ^prog_blk1 , ^scopelist10 )] : Frame_list `` ;
+val state_blk1 = ``(state_P4 FEMPTY ^frame_blk1 ^R): state``;
+
+val frame_blk2 = `` [("f", ^prog_blk2 , ^scopelist11 )] : Frame_list `` ;
+val state_blk2 = ``(state_P4 FEMPTY ( ^frame_blk2) ^R): state``;
+
+
 
 val test_stmt_block_enter =
-prove(`` stmt_red (^ctx_empty)(^prog6a) 
-                  (^state7)
-                  (^prog6b) 
-                  (^state8)  ``,
-RW.ONCE_RW_TAC[e_red_cases] >>
-EVAL_TAC>>
-SIMP_TAC list_ss []  
+prove(`` stmt_red (^ctx_empty) ^state_blk1 ^state_blk2 ``,
+STMT_SIMP >>
+EVAL_TAC
 );
 
 
- 
+val frame_blk3 = `` [("f", ^prog_blk1 , ^scopelist10 )] : Frame_list `` ;
+val state_blk3 = ``(state_P4 ^scope3 ^frame_blk3 ^R): state``;
+
+val frame_blk4 = `` [("f", ^prog_blk2 , ^scopelist11 )] : Frame_list `` ;
+val state_blk4 = ``(state_P4 ^scope3 ( ^frame_blk4) ^R): state``;
+
+(* test 1: transition for block enter*)
+val test_stmt_block_enter =
+prove(`` stmt_red (^ctx_empty) ^state_blk3 ^state_blk4 ``,
+STMT_SIMP >>
+EVAL_TAC
+);
+
+
+
+val frame_blk5 = `` [("f", ^prog_blk3 , ^scopelist11 )] : Frame_list `` ;
+val state_blk5 = ``(state_P4 ^scope3 ( ^frame_blk5) ^R): state``;
+
+
+ (* test 2: transition for block exec*)
 val test_stmt_block_exec =
-prove(`` stmt_red (^ctx_empty)(^prog6b) 
-                  (^state8)
-                  (^prog6c) 
-                  (^state9)  ``,
-REPEAT ( RW.ONCE_RW_TAC[e_red_cases] >>
-EVAL_TAC>>
-FULL_SIMP_TAC list_ss [] )
+prove(`` stmt_red (^ctx_empty) ^state_blk4 ^state_blk5  ``,
+RW_TAC (srw_ss()) [Once stmt_red_cases] >>
+EXISTS_TAC``^scope3`` >>
+STMT_SIMP 
 );
+
+
+(* test 3: transition for block exit*)
+val frame_blk6 = `` [("f", stmt_empty , ^scopelist10 )] : Frame_list `` ;
+val state_blk6 = ``(state_P4 ^scope3 ( ^frame_blk6) ^R): state``;
 
 
 val test_stmt_block_exit =
-prove(`` stmt_red (^ctx_empty)(^prog6c) 
-                  (^state9)
-                  (stmt_empty) 
-                  (^state7)  ``,
-RW.ONCE_RW_TAC[e_red_cases] >>
-REPEAT ( EVAL_TAC>>
-FULL_SIMP_TAC list_ss [] )
-);
-
-
-
-(*** stmt seq  statement reduction --concrete values -- ***)
-
-val prog7a =  ``(stmt_seq ^prog5 ^prog2)``;
-val prog7b =  ``(stmt_seq stmt_empty (^prog2))``;
-val prog7c =  ``(^prog2)``;
-val state7a = ``(state_tup (stacks_tup ^scopelist10 []) ^R): state``;
-val state7b = ``(state_tup (stacks_tup ^scopelist13 []) ^R): state``;
-val state7c = ``(state_tup (stacks_tup ^scopelist14 []) ^R): state``;
-
-val test_stmt_seq1 =
-prove(`` stmt_red (^ctx_empty) (^prog7a) 
-                  (^state7a)
-                  (^prog7b) 
-                  (^state7b)  ``,
-REPEAT (RW.ONCE_RW_TAC[e_red_cases] >>
-EVAL_TAC>>
-FULL_SIMP_TAC list_ss [])
-);
-
-
-val test_stmt_seq2 =
-prove(`` stmt_red (^ctx_empty) (^prog7b) 
-                  (^state7b)
-                  (^prog7c) 
-                  (^state7b)  ``,
-
-RW.ONCE_RW_TAC[e_red_cases] >>
-NTAC 6 DISJ2_TAC >>  DISJ1_TAC >>
-EXISTS_TAC``(stacks_tup
-         [FEMPTY |+ ("y",v_bit ([F],1),NONE) |+ ("x",v_bit ARB,NONE)] [])`` >>
-EVAL_TAC>>
-FULL_SIMP_TAC list_ss []
+prove(`` stmt_red (^ctx_empty) ^state_blk5 ^state_blk6 ``,
+STMT_SIMP >>
+EVAL_TAC
 );
 
 
 
 
+(*** transitions stmt reduction  ***)
 
-(*** transitions stmt reduction --concrete values -- ***)
-val prog9a =  ``stmt_trans (e_var "MoveNext") ``;
-val prog9b =  ``stmt_empty``;
-val prog9c =  ``stmt_trans (e_var "accept") ``;
-val prog9d =  ``stmt_trans (e_var "reject") ``;
-
-val state9a = ``(state_tup (stacks_tup ^scopelist10 []) ^R): state``;
-val state9b = ``(state_tup (stacks_tup ^scopelist10 []) (status_pars_next (pars_next_trans "MoveNext"))): state``;
-val state9c = ``(state_tup (stacks_tup ^scopelist10 []) ^Parse_Acc): state``;
-val state9d = ``(state_tup (stacks_tup ^scopelist10 []) ^Parse_Rej): state``;
+val prog_tra1 =  ``stmt_trans (e_v (v_str "MoveNext")) ``;
+val prog_tra2 =  ``stmt_trans (e_v (v_str "accept")) ``;
+val prog_tra3 =  ``stmt_trans (e_v (v_str "reject")) ``;
 
 
 
+val frame_tra1 = `` [("f", ^prog_tra1 , ^scopelist1 )] : Frame_list `` ;
+val state_tra1 = ``(state_P4 FEMPTY (^frame_tra1) ^R): state``;
+
+
+val frame_tra2 = `` [("f", stmt_empty , ^scopelist1 )] : Frame_list `` ;
+val state_tra2 = ``(state_P4 FEMPTY (^frame_tra2) (status_pars_next (pars_next_trans "MoveNext"))): state``;
+
+
+(* test 1: transition for stmt trans to non final*)
 val test_stmt_trans1 =
-prove(`` stmt_red (^ctx_empty) (^prog9a) 
-                  (^state9a)
-                  (^prog9b) 
-                  (^state9b)  ``,
-RW.ONCE_RW_TAC[e_red_cases] >>
-EVAL_TAC>>
-FULL_SIMP_TAC list_ss []
+prove(`` stmt_red (^ctx_empty) ^state_tra1 ^state_tra2   ``,
+STMT_SIMP >>
+EVAL_TAC
 );
 
 
+val frame_tra3 = `` [("f", ^prog_tra2 , ^scopelist1 )] : Frame_list `` ;
+val state_tra3 = ``(state_P4 ^scope8 (^frame_tra3) ^R): state``;
+
+
+val frame_tra4 = `` [("f", stmt_empty , ^scopelist1 )] : Frame_list `` ;
+val state_tra4 = ``(state_P4 ^scope8 (^frame_tra4) ^Parse_Acc): state``;
+
+
+(* test 2: transition for stmt trans to accept*)
 val test_stmt_trans2 =
-prove(`` stmt_red (^ctx_empty) (^prog9c) 
-                  (^state9a)
-                  (^prog9b) 
-                  (^state9c)  ``,
-RW.ONCE_RW_TAC[e_red_cases] >>
-EVAL_TAC>>
-FULL_SIMP_TAC list_ss []
+prove(`` stmt_red (^ctx_empty) ^state_tra3 ^state_tra4   ``,
+STMT_SIMP >>
+EVAL_TAC
 );
 
+
+val frame_tra5 = `` [("f", ^prog_tra3 , ^scopelist1 )] : Frame_list `` ;
+val state_tra5 = ``(state_P4 ^scope6 (^frame_tra5) ^R): state``;
+
+
+val frame_tra6 = `` [("f", stmt_empty , ^scopelist1 )] : Frame_list `` ;
+val state_tra6 = ``(state_P4 ^scope6 (^frame_tra6) ^Parse_Rej): state``;
+
+(* test 3: transition for stmt trans to accept*)
 val test_stmt_trans3 =
-prove(`` stmt_red (^ctx_empty) (^prog9d) 
-                  (^state9a)
-                  (^prog9b) 
-                  (^state9d)  ``,
-RW.ONCE_RW_TAC[e_red_cases] >>
-EVAL_TAC>>
-FULL_SIMP_TAC list_ss []
+prove(`` stmt_red (^ctx_empty) ^state_tra5 ^state_tra6   ``,
+STMT_SIMP >>
+EVAL_TAC
 );
-
 
 
 
@@ -410,223 +400,167 @@ FULL_SIMP_TAC list_ss []
 (*** verify  statement reduction --concrete values -- ***)
 
 (*Testing verify_e1 verify_e2 with both T and F evaluation *)
-val prog8a =  ``stmt_verify (^cond1) (e_v (v_err "PacketTooShort"))``;
-val prog8b =  ``stmt_verify (e_v (v_bool  T )) (e_v (v_err "PacketTooShort"))``;
-val prog8c =  ``stmt_verify (^cond2) (e_v (v_err "PacketTooShort"))``;
-val prog8d =  ``stmt_verify (e_v (v_bool  F )) (e_v (v_err "PacketTooShort"))``;
-val prog8e =  ``stmt_empty``;
-val prog8f =  ``stmt_seq (stmt_ass (lval_varname "parseError") ((e_v (v_err "PacketTooShort")))) (stmt_trans (e_var"reject"))``;
+
+val prog_ver1 =  ``stmt_verify (^cond1) (e_v (v_err "PacketTooShort"))``;
+val prog_ver2 =  ``stmt_verify (e_v (v_bool  T )) (e_v (v_err "PacketTooShort"))``;
+
+val prog_ver3 =  ``stmt_verify (^cond2) (e_v (v_err "PacketTooShort"))``;
+val prog_ver4 =  ``stmt_verify (e_v (v_bool  F )) (e_v (v_err "PacketTooShort"))``;
+
+val prog_ver5 =  ``stmt_seq (stmt_ass (lval_varname (varn_name "parseError")) ((e_v (v_err "PacketTooShort")))) (stmt_trans (e_v (v_str "reject")))``;
 
 
+val frame_ver1 = `` [("f", ^prog_ver1 , ^scopelist2 )] : Frame_list `` ;
+val state_ver1 = ``(state_P4 ^scope8 (^frame_ver1) ^R): state``;
 
 
-val state8a = ``(state_tup (stacks_tup ^scopelist10 []) ^R): state``;
-val state8b = ``(state_tup (stacks_tup ^scopelist10 []) ^R): state``;
+val frame_ver2 = `` [("f", ^prog_ver2 , ^scopelist2 )] : Frame_list `` ;
+val state_ver2 = ``(state_P4 ^scope8 (^frame_ver2) ^R): state``;
 
 
+(* test 1: transition for stmt verify e e -> verify T e*)
 
-(*Testing verify_e1*)
 val test_stmt_verify1 =
-prove(`` stmt_red (^ctx_empty)(^prog8a) 
-                  (^state8a)
-                  (^prog8b) 
-                  (^state8a)  ``,
-REPEAT (RW.ONCE_RW_TAC[e_red_cases] >>
-EVAL_TAC>>
-FULL_SIMP_TAC list_ss [])
+prove(`` stmt_red (^ctx_empty) ^state_ver1 ^state_ver2  ``,
+STMT_SIMP >>
+EXISTS_TAC``[] : ((string # stmt # scopes_stack) list) `` >>
+EXISTS_TAC``(e_v (v_bool T)) `` >>
+EXP_SIMP
 );
 
+
+val frame_ver3 = `` [("f", stmt_empty , ^scopelist2 )] : Frame_list `` ;
+val state_ver3 = ``(state_P4 ^scope8 (^frame_ver3) ^R): state``;
+
+
+(* test 2: transition for stmt verify T e -> empty*)
 val test_stmt_verify2 =
-prove(`` stmt_red (^ctx_empty)(^prog8c) 
-                  (^state8a)
-                  (^prog8d) 
-                  (^state8a)  ``,
-REPEAT (RW.ONCE_RW_TAC[e_red_cases] >>
-EVAL_TAC>>
-FULL_SIMP_TAC list_ss [])
+prove(`` stmt_red (^ctx_empty) ^state_ver2 ^state_ver3 ``,
+STMT_SIMP
 );
 
 
-(*Testing verify_3*)
+
+
+val frame_ver4 = `` [("f", ^prog_ver3 , ^scopelist2 )] : Frame_list `` ;
+val state_ver4 = ``(state_P4 ^scope8 (^frame_ver4) ^R): state``;
+
+val frame_ver5 = `` [("f", ^prog_ver4 , ^scopelist2 )] : Frame_list `` ;
+val state_ver5 = ``(state_P4 ^scope8 (^frame_ver5) ^R): state``;
+
+(* test 3: transition for stmt verify e e -> verify F e*)
 val test_stmt_verify3 =
-prove(`` stmt_red (^ctx_empty)(^prog8b) 
-                  (^state8a)
-                  (^prog8e) 
-                  (^state8a)  ``,
-RW.ONCE_RW_TAC[e_red_cases] >>
-EVAL_TAC>>
-FULL_SIMP_TAC list_ss []
+prove(`` stmt_red (^ctx_empty) ^state_ver4 ^state_ver5  ``,
+STMT_SIMP >>
+EXISTS_TAC``[] : ((string # stmt # scopes_stack) list) `` >>
+EXISTS_TAC``(e_v (v_bool F)) `` >>
+EXP_SIMP >>
+EVAL_TAC
 );
 
 
-(*Testing verify_4 *)
+val frame_ver6 = `` [("f", ^prog_ver5 , ^scopelist2 )] : Frame_list `` ;
+val state_ver6 = ``(state_P4 ^scope8 (^frame_ver6) ^R): state``;
 
+
+(* test 4: transition for stmt verify F e -> parserError = errmsg ; trans rej*)
 val test_stmt_verify4 =
-prove(`` stmt_red (^ctx_empty)(^prog8d) 
-                  (^state8a)
-                  (^prog8f) 
-                  (^state8a)  ``,
-RW.ONCE_RW_TAC[e_red_cases] >>
-EVAL_TAC>>
-FULL_SIMP_TAC list_ss []  
+prove(`` stmt_red (^ctx_empty) ^state_ver5 ^state_ver6 ``,
+STMT_SIMP
 );
 
 
-(*Testing verify_4 the whole execustion*)
-val prog8g =  ``stmt_seq stmt_empty (stmt_trans (e_var"reject"))``;
-val prog8h =  ``(stmt_trans (e_var"reject"))``;
-val state10a = ``(state_tup (stacks_tup ^scopelist15 []) ^R): state``;
-val state10b = ``(state_tup (stacks_tup ^scopelist16 []) ^R): state``;
-val state10c = ``(state_tup (stacks_tup ^scopelist16 []) ^Parse_Rej): state``;
 
+(*Testing verify_4 the whole execustion SEQ*)
 
-val test_stmt_verify5 =
-prove(``(stmt_red (^ctx_empty) (^prog8d) 
-                  (^state10a)
-                  (^prog8f) 
-                  (^state10a))
-		  /\
-	(stmt_red (^ctx_empty) (^prog8f) 
-                  (^state10a)
-                  (^prog8g) 
-                  (^state10b))
-		  /\
-	(stmt_red (^ctx_empty) (^prog8g) 
-                  (^state10b)
-                  (^prog8h) 
-                  (^state10b))
-		  /\
-	 (stmt_red (^ctx_empty) (^prog8h) 
-                  (^state10b)
-                  (stmt_empty) 
-                  (^state10c))	  		  
+val prog_ver6 =  ``stmt_seq stmt_empty (stmt_trans (e_v (v_str "reject")))``;
+val prog_ver7 =  ``(stmt_trans (e_v (v_str "reject")))``;
+
+val frame_ver7 = `` [("f", ^prog_ver6 , ^scopelist15 )] : Frame_list `` ;
+val state_ver7 = ``(state_P4 ^scope8 (^frame_ver7) ^R): state``;
+
+val frame_ver8 = `` [("f", ^prog_ver5 , ^scopelist15 )] : Frame_list `` ;
+val state_ver8 = ``(state_P4 ^scope8 (^frame_ver8) ^R): state``;
+
+val frame_ver9 = `` [("f", ^prog_ver6 , ^scopelist16 )] : Frame_list `` ;
+val state_ver9 = ``(state_P4 ^scope8 (^frame_ver9) ^R): state``;
+
+val frame_ver10 = `` [("f", ^prog_ver7 , ^scopelist16 )] : Frame_list `` ;
+val state_ver10 = ``(state_P4 ^scope8 (^frame_ver10) ^R): state``;
+
+val frame_ver11 = `` [("f", stmt_empty , ^scopelist16 )] : Frame_list `` ;
+val state_ver11 = ``(state_P4 ^scope8 (^frame_ver11) ^Parse_Rej): state``;
+
+val test_stmt_verifyFULL =
+prove(``(stmt_red (^ctx_empty) ^state_ver7 ^state_ver8)
+    /\  (stmt_red (^ctx_empty) ^state_ver8 ^state_ver9)
+    /\  (stmt_red (^ctx_empty) ^state_ver9 ^state_ver10)
+    /\  (stmt_red (^ctx_empty) ^state_ver10 ^state_ver11)
 ``,
 CONJ_TAC >| [
-RW.ONCE_RW_TAC[e_red_cases] >>
-EVAL_TAC>>
-FULL_SIMP_TAC list_ss []
+STMT_SIMP >>
+DISJ1_TAC>>
+ EXISTS_TAC``[] : Frame_list `` >>
+ EXISTS_TAC``(stmt_ass (lval_varname "parseError")
+             (e_v (v_err "PacketTooShort")))`` >>
+ EXISTS_TAC``^scopelist15`` >>
+ EVAL_TAC
+ 
+,
+ CONJ_TAC >| [
+ STMT_SIMP >>
+ DISJ1_TAC >>
+ EXISTS_TAC``[] : ((string # stmt # scopes_stack) list) `` >>
+ EXISTS_TAC``stmt_empty`` >>
+ EXISTS_TAC``^scopelist16`` >>
+ EVAL_TAC >>
+ STMT_SIMP >>
+ DISJ1_TAC >>
+ EXISTS_TAC``[^scope8]++^scopelist16`` >>
+ EVAL_TAC>>
+ FULL_SIMP_TAC list_ss [FUPDATE_EQ]
 ,
 CONJ_TAC >| [
-NTAC 3 (RW.ONCE_RW_TAC[e_red_cases] >>
-EVAL_TAC>>
-FULL_SIMP_TAC list_ss [FUPDATE_EQ])
+STMT_SIMP
 ,
-CONJ_TAC >| [
-RW.ONCE_RW_TAC[e_red_cases] >>
-NTAC 6 DISJ2_TAC >>  DISJ1_TAC >>
-EXISTS_TAC``(stacks_tup
-            [FEMPTY |+ ("z",v_bit ([T],1),NONE) |+
-             ("parseError",v_err "PacketTooShort",NONE)] [])`` >>
-EVAL_TAC
-,
-RW.ONCE_RW_TAC[e_red_cases] >>
-EVAL_TAC>>
-FULL_SIMP_TAC list_ss []
+STMT_SIMP
 ]]]
 );
 
 
 
 
-(*** Parser reductions --concrete values -- ***)
+(*** stmt seq  statement reduction --concrete values -- ***)
+val prog_seq1  = ``(stmt_declare "x"  (t_base bt_bit) )``;
+val prog_seq2  = ``(stmt_ass (lval_varname "x") (e_v (v_bit ([F], 1))))``;
+val prog_seq3 =  ``(stmt_seq ^prog_seq1 ^prog_seq2)``;
+val prog_seq4 =  ``(stmt_seq stmt_empty ^prog_seq2)``;
 
-val pars_map = ``(FEMPTY |+ ("start", stmt_seq (^prog8b)  (stmt_trans (e_var "p_ipv4")))
-                         |+ ("p_ipv4", (^prog2) ))``;
-
-val ctx1 = ``(FEMPTY, FEMPTY, ^pars_map, FEMPTY, empty_ctrl):ctx``;
-
-val state11a = ``(state_tup (stacks_tup ^scopelist2 []) ^R): state``;
-val state11b = ``(state_tup (stacks_tup ^scopelist1 []) ^R): state``;
-val state11c = ``(state_tup (stacks_tup ^scopelist1 []) ^Parse_Rej): state``;
-val state11d = ``(state_tup (stacks_tup ^scopelist1 []) ^Parse_Acc): state``;
-
-val test_pars_sem1 =
-prove(`` pars_red (^ctx1) (stmt_seq (^prog8b)  (stmt_trans (e_var "p_ipv4"))) 
-                  (^state11a)  
-                  (stmt_seq stmt_empty  (stmt_trans (e_var "p_ipv4")))
-                  (^state11a) ``,
-REPEAT (RW.ONCE_RW_TAC[pars_red_cases, e_red_cases] >>
-EVAL_TAC>>
-FULL_SIMP_TAC list_ss [])
-);
+val frame_seq1 = `` [("f", ^prog_seq3 , ^scopelist10 )] : Frame_list `` ;
+val state_seq1 = ``(state_P4 ^scope8 (^frame_seq1) ^R): state``;
 
 
-val test_pars_sem2 =
-prove(`` pars_red (^ctx1) (stmt_seq stmt_empty  (stmt_trans (e_var "p_ipv4"))) 
-                  (^state11a)  
-                  (stmt_trans (e_var "p_ipv4"))
-                  (^state11a) ``,
-RW.ONCE_RW_TAC[pars_red_cases] >>
+val frame_seq2 = `` [("f", ^prog_seq4 , ^scopelist13 )] : Frame_list `` ;
+val state_seq2 = ``(state_P4 ^scope8 (^frame_seq2) ^R): state``;
+
+
+(* test 1: transition for    seq dec ; x = F -> seq empty ; x= F *)
+val test_stmt_seq1 =
+prove(`` stmt_red (^ctx_empty) ^state_seq1 ^state_seq2 ``,
+STMT_SIMP >>
 DISJ1_TAC >>
-EVAL_TAC>>
-NTAC 2 (EXISTS_TAC``stacks_tup [FEMPTY |+ ("x",v_bit ([T],1),NONE)] []``) >>
-EVAL_TAC>>
-RW.ONCE_RW_TAC[e_red_cases] >>
-NTAC 6 DISJ2_TAC >>  DISJ1_TAC >>
-EXISTS_TAC``(stacks_tup [FEMPTY |+ ("x",v_bit ([T],1),NONE)] [])`` >>
+RW_TAC (srw_ss()) [Once stmt_red_cases] >>
 EVAL_TAC
 );
 
 
-val test_pars_sem3 =
-prove(`` pars_red (^ctx1)(stmt_trans (e_var "p_ipv4"))
-                  (^state11a)
-		  (^prog2)
-                  (^state11a) ``,
-NTAC 2 (RW.ONCE_RW_TAC[pars_red_cases, e_red_cases] >>
-EVAL_TAC>>
-FULL_SIMP_TAC list_ss []) >>
-EVAL_TAC
-);
+(* test 2: transition for    seq empty ; x= F -> x = F*)
+val frame_seq3 = `` [("f", ^prog_seq2 , ^scopelist13 )] : Frame_list `` ;
+val state_seq3 = ``(state_P4 ^scope8 (^frame_seq3) ^R): state``;
 
-
-
-val test_pars_sem4 =
-prove(`` pars_red (^ctx1) (^prog2)
-                  (^state11a)
-		  (stmt_trans (e_var "reject"))
-                  (^state11b) ``,
-RW.ONCE_RW_TAC[pars_red_cases] >>
-EVAL_TAC>>
-FULL_SIMP_TAC list_ss [] >>
-NTAC 2 (DISJ2_TAC) >>
-RW.ONCE_RW_TAC[e_red_cases] >>
-EVAL_TAC>>
-FULL_SIMP_TAC std_ss []>>
-EVAL_TAC>>
-SIMP_TAC std_ss [FUPDATE_EQ]
-
-);
-
-
-val test_pars_sem5 =
-prove(`` pars_t_red (^ctx1)(stmt_trans (e_var "reject"))
-                    (^state11b)
-		    (^state11c) ``,
-RW.ONCE_RW_TAC[pars_t_red_cases] >>
-EVAL_TAC>>
-FULL_SIMP_TAC list_ss [] >>
-EXISTS_TAC``stmt_empty`` >>
-RW.ONCE_RW_TAC[e_red_cases] >>
-EVAL_TAC>>
-FULL_SIMP_TAC std_ss []>>
-EVAL_TAC
-);
-
-
-(*extra check for accpet*)
-val test_pars_sem5 =
-prove(`` pars_t_red (^ctx1) (stmt_trans (e_var "accept"))
-                  (^state11b)
-		  (^state11d) ``,
-RW.ONCE_RW_TAC[pars_t_red_cases] >>
-EVAL_TAC>>
-FULL_SIMP_TAC list_ss [] >>
-EXISTS_TAC``stmt_empty`` >>
-RW.ONCE_RW_TAC[e_red_cases] >>
-EVAL_TAC>>
-FULL_SIMP_TAC std_ss []>>
-EVAL_TAC
+val test_stmt_seq2 =
+prove(`` stmt_red (^ctx_empty) ^state_seq2 ^state_seq3  ``,
+STMT_SIMP 
 );
 
 
@@ -635,38 +569,50 @@ EVAL_TAC
 
 (*** lookup expression  reduction --concrete values -- ***)
 
-val state_e1 = ``(stacks_tup (^scopelist8) [])``;
+(* test 1: lookup e current frames stack while global empty*)
+val test_e_lookup1 =
+prove(`` e_red  (^ctx_empty) FEMPTY ^scopelist8
+               (e_var (varn_name"x")) (e_v (v_bit ([F],1))) ([]) ``,
+NTAC 2 EXP_SIMP
+);
 
-val test_e_lookup =
-prove(`` e_red    (^ctx_empty) (e_var "x") 
-                  (^state_e1)  (^R)
-                  (e_v (v_bit ([F],1))) 
-                  (^state_e1)  (^R) ``,
-RW.ONCE_RW_TAC[e_red_cases, lookup_vexp_def] >>
-NTAC 2 (EVAL_TAC>>
-FULL_SIMP_TAC list_ss []  )
+(* test 2: lookup e current frames stack while global non empty*)
+val test_e_lookup2 =
+prove(`` e_red  (^ctx_empty) ^scope1 ^scopelist8
+               (e_var (varn_name"x")) (e_v (v_bit ([F],1))) ([]) ``,
+NTAC 2 EXP_SIMP
+);
+
+
+(* test 3: lookup varn_star current frames stack while global non empty*)
+val test_e_lookup3 =
+prove(`` e_red  (^ctx_empty) FEMPTY ^scopelist30
+               (e_var (varn_star)) (e_v (v_bit ([F; F],2))) ([]) ``,
+NTAC 2 EXP_SIMP
 );
 
 
 
 
-(*** more on assignment (struct, header field and null)  reduction --concrete values -- ***)
-val state12a  = ``(state_tup (stacks_tup ^scopelist7 []) ^R): state``;
-val prog10a   = ``stmt_ass lval_null (e_v (v_bit ([T],1)))``;
-val prog10b   = ``stmt_ass (lval_field (lval_varname "f") "f") ``;
 
-(*tests of assignment null*)
+(*** more on assignment null  ***)
+val prog_null1   = ``stmt_ass lval_null (e_v (v_bit ([T],1)))``;
+
+
+val frame_null1 = `` [("f", ^prog_null1 , ^scopelist7 )] : Frame_list `` ;
+val state_null1 = ``(state_P4 ^scope3 (^frame_null1) ^R): state``;
+
+val frame_null2 = `` [("f", stmt_empty , ^scopelist7 )] : Frame_list `` ;
+val state_null2 = ``(state_P4 ^scope3 (^frame_null2) ^R): state``;
+
+
+(* test 1: assign to null changes nothing*)
 val test_stmt_ass_null =
-prove(`` stmt_red (^ctx1) (^prog10a) 
-                  (^state12a)
-                  (stmt_empty) 
-                  (^state12a) ``,
-RW.ONCE_RW_TAC[e_red_cases, lookup_vexp_def] >>
-EVAL_TAC>>
-FULL_SIMP_TAC list_ss []
+prove(`` stmt_red (^ctx_empty) ^state_null1 ^state_null2 ``,
+STMT_SIMP
 );
 
-(*TODO: Ask Didrik about the records and header representation?*)
+
 
 
 
@@ -676,71 +622,77 @@ FULL_SIMP_TAC list_ss []
 
 (****copy_in IN values aka func_call_args rule ****)
 
-val func_sig1 = ``(FEMPTY |+ ("Add1", (stmt_empty , [("y",d_in)] )))``;
-val ctx2 = ``(FEMPTY, ^func_sig1, FEMPTY, FEMPTY, empty_ctrl):ctx``;
-val prog_call1a = ``(e_func_call "Add1" [e_var "x"]) ``;
-val prog_call1b = ``(e_func_call "Add1" [(e_v (v_bit ([F],1)))]) ``;
-val stacks_call1a  = ``(stacks_tup ^scopelist1 [])``;
+val func_sig1 = ``(FEMPTY |+ ("Add1", (stmt_empty , [("y",d_in)] ))): func_map``;
+val ctx1 = ``(FEMPTY, ^func_sig1, FEMPTY, FEMPTY, empty_ctrl):ctx``;
 
+val prog_call1 = ``(e_func_call "Add1" [e_var (varn_name"x")]) ``;
+val prog_call2 = ``(e_func_call "Add1" [(e_v (v_bit ([F],1)))]) ``;
 
-
+(* test 1: test exp red : call Add1 (x) ~> call Add1 (1)
+where the arg is IN i.e. not copied in*)
 
 val test_COPYIN1 =
-prove(`` e_red    (^ctx2)(^prog_call1a) 
-                  (^stacks_call1a) (^R)
-                  (^prog_call1b) 
-                  (^stacks_call1a) (^R)``,
+prove(`` e_red  (^ctx1) ^scope2 [FEMPTY]
+           (^prog_call1)
+	   (^prog_call2)  ([]) ``,
+	   
 RW.ONCE_RW_TAC[e_red_cases] >>
 EVAL_TAC>>
 FULL_SIMP_TAC list_ss [] >>
-EXISTS_TAC ``[( e_var "x", (e_v (v_bit ([F],1))) , "y" , d_in)]`` >>
+EXISTS_TAC ``[( e_var( varn_name "x"), (e_v (v_bit ([F],1))) , "y" , d_in)]`` >>
 EXISTS_TAC ``(stmt_empty)`` >>
 RW.ONCE_RW_TAC[e_red_cases] >>
-NTAC 3 (EVAL_TAC>>
+NTAC 2 (EVAL_TAC>>
 FULL_SIMP_TAC list_ss [])
 );
 
 
 
 
-val func_sig2 = ``(FEMPTY |+ ("Add1", (stmt_empty , [("y",d_none)] )))``;
-val ctx3 = ``(FEMPTY, ^func_sig2, FEMPTY, FEMPTY, empty_ctrl):ctx``;
+
+(* test 2: test exp red : call Add1 (x) ~> call Add1 (1)
+where the arg is IN i.e. not copied in*)
+
+val func_sig2 = ``(FEMPTY |+ ("Add1", (stmt_empty , [("y",d_none)] ))): func_map``;
+val ctx2 = ``(FEMPTY, ^func_sig2, FEMPTY, FEMPTY, empty_ctrl):ctx``;
 
 val test_COPYIN2 =
-prove(`` e_red    (^ctx3)(^prog_call1a) 
-                  (^stacks_call1a) (^R)
-                  (^prog_call1b) 
-                  (^stacks_call1a) (^R)``,
+prove(`` e_red  (^ctx2) ^scope2 [FEMPTY]
+           (^prog_call1)
+	   (^prog_call2)  ([]) ``,
 RW.ONCE_RW_TAC[e_red_cases] >>
 EVAL_TAC>>
 FULL_SIMP_TAC list_ss [] >>
-EXISTS_TAC ``[( e_var "x", (e_v (v_bit ([F],1))) , "y" , d_none)]`` >>
+EXISTS_TAC ``[( e_var ( varn_name "x"), (e_v (v_bit ([F],1))) , "y" , d_none)]`` >>
 EXISTS_TAC ``(stmt_empty)`` >>
 RW.ONCE_RW_TAC[e_red_cases] >>
-NTAC 3 (EVAL_TAC>>
+NTAC 2 (EVAL_TAC>>
 FULL_SIMP_TAC list_ss [])
 );
 
 
 
 
-(*two arguments call  out in *)
+(* test 3: test exp red : call Add1 (y, x) ~> call Add1 (y ,1)
+where y is OUT so it is copied out, thus we do not evaluate it in the first swipe
+and   x is IN so it will be the first value to evaluate and not copied in *)
+
 val func_sig3 = ``(FEMPTY |+ ("Add1", (stmt_empty , [("a",d_out); ("b", d_in)] )))``;
-val ctx4 = ``(FEMPTY, ^func_sig3, FEMPTY, FEMPTY, empty_ctrl):ctx``;
-val prog_call2a = ``(e_func_call "Add1" [e_var "y"; e_var "x"]) ``; (*call the function with x,y*)
-val prog_call2b = ``(e_func_call "Add1" [e_var "y"; (e_v (v_bit ([F],1)))]) ``;
+val ctx3 = ``(FEMPTY, ^func_sig3, FEMPTY, FEMPTY, empty_ctrl):ctx``;
+val prog_call3 = ``(e_func_call "Add1" [e_var (varn_name "y"); e_var (varn_name "x")]) ``; (*call the function with x,y*)
+val prog_call4 = ``(e_func_call "Add1" [e_var (varn_name "y"); (e_v (v_bit ([F],1)))]) ``;
 
 
 val test_COPYIN3 =
-prove(`` e_red    (^ctx4)(^prog_call2a) 
-                  (^stacks_call1a) (^R)
-                  (^prog_call2b) 
-                  (^stacks_call1a) (^R)``,
+prove(`` e_red (^ctx3) ^scope2 [FEMPTY]
+           (^prog_call3)
+	   (^prog_call4)  ([])``,
+	   
 RW.ONCE_RW_TAC[e_red_cases] >>
 EVAL_TAC>>
 FULL_SIMP_TAC list_ss [] >>
-EXISTS_TAC ``[( e_var "y", e_var "y"            , "a" , d_out);
-              ( e_var "x",(e_v (v_bit ([F],1))) , "b" , d_in)]`` >>
+EXISTS_TAC ``[( e_var (varn_name "y"), e_var (varn_name "y") , "a" , d_out);
+              ( e_var (varn_name "x"),(e_v (v_bit ([F],1))) , "b" , d_in)]`` >>
 EXISTS_TAC ``(stmt_empty)`` >>
 
 RW.ONCE_RW_TAC[e_red_cases] >>
@@ -750,23 +702,25 @@ FULL_SIMP_TAC list_ss [])
 
 
 
-(*two arguments call  none out*)
+(* test 4: test exp red : call Add1 (x, y) ~> call Add1 (1 ,y)
+where x is NONE so it is not copied out, thus we do evaluate it in the first swipe
+and   y is OUT  *)
+
 val func_sig4 = ``(FEMPTY |+ ("Add1", (stmt_empty , [("a",d_none); ("b", d_out)] )))``;
-val ctx5 = ``(FEMPTY, ^func_sig4, FEMPTY, FEMPTY, empty_ctrl):ctx``;
-val prog_call3a = ``(e_func_call "Add1" [ e_var "x"; e_var "y"]) ``; (*call the function with a,b*)
-val prog_call3b = ``(e_func_call "Add1" [(e_v (v_bit ([F],1))); e_var "y"]) ``;
+val ctx4 = ``(FEMPTY, ^func_sig4, FEMPTY, FEMPTY, empty_ctrl):ctx``;
+val prog_call5 = ``(e_func_call "Add1" [ e_var (varn_name "x"); e_var (varn_name "y")]) ``; (*call the function with a,b*)
+val prog_call6 = ``(e_func_call "Add1" [(e_v (v_bit ([F],1))); e_var (varn_name "y")]) ``;
 
 
 val test_COPYIN4 =
-prove(`` e_red    (^ctx5)(^prog_call3a) 
-                  (^stacks_call1a) (^R)
-                  (^prog_call3b) 
-                  (^stacks_call1a) (^R)``,
+prove(``e_red (^ctx4) ^scope2 [FEMPTY]
+           (^prog_call5)
+	   (^prog_call6)  ([])``,
 RW.ONCE_RW_TAC[e_red_cases] >>
 EVAL_TAC>>
 FULL_SIMP_TAC list_ss [] >>
-EXISTS_TAC ``[( e_var "x",(e_v (v_bit ([F],1))) , "a" , d_none);
-              ( e_var "y",    e_var"y"          , "b" , d_out)]`` >>
+EXISTS_TAC ``[( e_var (varn_name "x"),(e_v (v_bit ([F],1))) , "a" , d_none);
+              ( e_var (varn_name "y"), e_var (varn_name "y") , "b" , d_out)]`` >>
 EXISTS_TAC ``(stmt_empty)`` >>
 
 RW.ONCE_RW_TAC[e_red_cases] >>
@@ -776,69 +730,61 @@ FULL_SIMP_TAC list_ss [])
 
 
 
-(*two arguments call none in with expression operations*)
+(* test 5 + 6: two arguments call NONE and IN reduction sequence*)
 val func_sig5 = ``(FEMPTY |+ ("Add1", (stmt_empty , [("a",d_none); ("b", d_in)] )))``;
-val ctx6 = ``(FEMPTY, ^func_sig5, FEMPTY, FEMPTY, empty_ctrl):ctx``;
-val stacks_call4a  = ``(stacks_tup ^scopelist17 [])``;
-val prog_call4a = ``(e_func_call "Add1" [ e_var "x" ; e_var "y"]) ``; 
-val prog_call4b = ``(e_func_call "Add1" [(e_v (v_bit ([F],1))); e_var "y"]) ``;
-val prog_call4c = ``(e_func_call "Add1" [(e_v (v_bit ([F],1))); (e_v (v_bit ([T],1)))]) ``;
+val ctx5 = ``(FEMPTY, ^func_sig5, FEMPTY, FEMPTY, empty_ctrl):ctx``;
+
+
+val prog_call7 = ``(e_func_call "Add1" [ e_var (varn_name "x") ; e_var (varn_name "y")]) ``; 
+val prog_call8 = ``(e_func_call "Add1" [(e_v (v_bit ([F],1))); e_var (varn_name "y")]) ``;
+val prog_call9 = ``(e_func_call "Add1" [(e_v (v_bit ([F],1))); (e_v (v_bit ([T],1)))]) ``;
+
 
 val test_COPYIN5 =
-prove(`` e_red   (^ctx6) (^prog_call4a) 
-                  (^stacks_call4a) (^R)
-                  (^prog_call4b) 
-                  (^stacks_call4a) (^R)``,
-RW.ONCE_RW_TAC[e_red_cases] >>
-EVAL_TAC>>
-FULL_SIMP_TAC list_ss [] >>
-EXISTS_TAC ``[( e_var "x",(e_v (v_bit ([F],1))) , "a" , d_none);
-              ( e_var "y",e_var "y" , "b" , d_in)]`` >>
+prove(`` e_red (^ctx5) ^scope11 [FEMPTY]
+           (^prog_call7)
+	   (^prog_call8)  ([])``,
+EXP_SIMP >>
+EXISTS_TAC ``[(e_var (varn_name "x"),(e_v (v_bit ([F],1))) , "a" , d_none);
+              (e_var (varn_name "y"),e_var (varn_name "y"), "b" , d_in)]`` >>
 EXISTS_TAC ``(stmt_empty)`` >>
 
 
 RW.ONCE_RW_TAC[e_red_cases] >>
-REPEAT (EVAL_TAC>>
-FULL_SIMP_TAC list_ss [])
+REPEAT (EXP_SIMP )
 );
 
 
 
 val test_COPYIN6 =
-prove(`` e_red    (^ctx6)(^prog_call4b) 
-                  (^stacks_call4a) (^R)
-                  (^prog_call4c) 
-                  (^stacks_call4a) (^R)``,
-RW.ONCE_RW_TAC[e_red_cases] >>
-EVAL_TAC>>
-FULL_SIMP_TAC list_ss [] >>
+prove(`` e_red (^ctx5) ^scope11 [FEMPTY]
+           (^prog_call8)
+	   (^prog_call9)  ([])``,
+EXP_SIMP >>
 EXISTS_TAC ``[( (e_v (v_bit ([F],1))),(e_v (v_bit ([F],1))) , "a" , d_none);
-              ( e_var "y"            ,(e_v (v_bit ([T],1))) , "b" , d_in)]`` >>
+              ( e_var (varn_name "y"),(e_v (v_bit ([T],1))) , "b" , d_in)]`` >>
 EXISTS_TAC ``(stmt_empty)`` >>
 
 RW.ONCE_RW_TAC[e_red_cases] >>
-REPEAT (EVAL_TAC>>
-FULL_SIMP_TAC list_ss [])
+REPEAT (EXP_SIMP )
 );
 
 
 
+(* test 7: one arg red with expression operation*)
 
-val prog_call5a = ``(e_func_call "Add1" [e_binop (e_var "x") binop_add (e_var "y")]) ``; 
-val prog_call5b = ``(e_func_call "Add1" [e_binop (e_v (v_bit ([F],1))) binop_add (e_var "y")]) ``; 
+val prog_call10 = ``(e_func_call "Add1" [e_binop (e_var (varn_name "x")) binop_add (e_var (varn_name "y"))]) ``; 
+val prog_call11 = ``(e_func_call "Add1" [e_binop (e_v (v_bit ([F],1))) binop_add  (e_var (varn_name "y"))]) ``; 
 val func_sig6 = ``(FEMPTY |+ ("Add1", (stmt_empty , [("a",d_in)] )))``;
-val ctx7 = ``(FEMPTY, ^func_sig6, FEMPTY, FEMPTY, empty_ctrl):ctx``;
+val ctx6 = ``(FEMPTY, ^func_sig6, FEMPTY, FEMPTY, empty_ctrl):ctx``;
 
 val test_COPYIN7 =
-prove(`` e_red    (^ctx7)(^prog_call5a) 
-                  (^stacks_call4a) (^R)
-                  (^prog_call5b) 
-                  (^stacks_call4a) (^R)``,
-RW.ONCE_RW_TAC[e_red_cases] >>
-EVAL_TAC>>
-FULL_SIMP_TAC list_ss [] >>
-EXISTS_TAC ``[(e_binop (e_var "x") binop_add (e_var "y")),
-               e_binop (e_v (v_bit ([F],1))) binop_add (e_var "y")
+prove(`` e_red (^ctx6) ^scope11 [FEMPTY]
+           (^prog_call10)
+	   (^prog_call11)  ([])``,
+EXP_SIMP >>
+EXISTS_TAC ``[(e_binop  (e_var (varn_name "x")) binop_add  (e_var (varn_name "y"))),
+               e_binop (e_v (v_bit ([F],1))) binop_add  (e_var (varn_name "y"))
 	       , "a"
 	       , d_in]`` >>
 EXISTS_TAC ``(stmt_empty)`` >>
@@ -849,10 +795,7 @@ EVAL_TAC>>
 FULL_SIMP_TAC list_ss []
 ) >>
 
-REPEAT (
-RW.ONCE_RW_TAC[e_red_cases] >>
-EVAL_TAC>>
-FULL_SIMP_TAC list_ss [])
+REPEAT (EXP_SIMP)
 );
 
 
@@ -860,189 +803,164 @@ FULL_SIMP_TAC list_ss [])
 
 val Fn = ``called_function_name_function_name``; 
 
-(****copy_in IN values aka func_call_newframe rule ****)
+(****copy_in OUT values aka func_call_newframe rule ****)
+(* test 8: copy_in IN values aka func_call_newframe rule*)
 
 val func_sig7 = ``(FEMPTY |+ ("Add1", (stmt_empty , [("y",d_in)] )))``;
-val ctx8 = ``(FEMPTY, ^func_sig7, FEMPTY, FEMPTY, empty_ctrl):ctx``;
-val prog_call1b = ``(e_func_call "Add1" [(e_v (v_bit ([F],1)))]) ``;
-val stacks_call5a  = ``(stacks_tup ^scopelist1 [])``;
-val stacks_call5b  = ``(stacks_tup ^scopelist19 [([] , ^Fn "Add1")])``;
-(*we can't add (^scopelist1 , ^Fn "Add1") here in the call stack because we are calling from main*)
+val ctx7 = ``(FEMPTY, ^func_sig7, FEMPTY, FEMPTY, empty_ctrl):ctx``;
+
+val prog_call12 = ``(e_func_call "Add1" [(e_v (v_bit ([F],1)))]) ``;
 
 
 val test_NEWFRAME1 =
-prove(`` e_red    (^ctx8)(^prog_call1b) 
-                  (^stacks_call5a) (^R)
-                  (e_func_exec stmt_empty) 
-                  (^stacks_call5b) (^R)``,
+prove(`` e_red (^ctx7) ^scope2 [FEMPTY]
+                  (^prog_call12) 
+                  (e_var varn_star) [("Add1", stmt_empty , [^scope13] )]``,
 
-RW.ONCE_RW_TAC[e_red_cases] >>
-EVAL_TAC>>
-
-DISJ2_TAC >> DISJ1_TAC >>
+EXP_SIMP >>
 EXISTS_TAC ``[( (e_v (v_bit ([F],1)))
 	       , "y"
 	       , d_in)]`` >>
-REPEAT (EVAL_TAC>>
-FULL_SIMP_TAC list_ss [] )
-
+EVAL_TAC>>
+FULL_SIMP_TAC list_ss []
 );
 
 
-
+(******************************************************)
 (****copy_in OUT values aka func_call_newframe rule ****)
+(* test 9: copy_in OUT values aka func_call_newframe rule*)
 
 val func_sig8 = ``(FEMPTY |+ ("Add1", (stmt_empty , [("y",d_out)] )))``;
-val ctx9 = ``(FEMPTY, ^func_sig8, FEMPTY, FEMPTY, empty_ctrl):ctx``;
-val prog_call6a = ``(e_func_call "Add1" [e_var "x"]) ``;
-val stacks_call6a  = ``(stacks_tup ^scopelist1 [])``;
-val stacks_call6b  = ``(stacks_tup ^scopelist20 [([] , ^Fn "Add1")])``;
+val ctx8 = ``(FEMPTY, ^func_sig8, FEMPTY, FEMPTY, empty_ctrl):ctx``;
+
+val prog_call13 = ``(e_func_call "Add1" [e_var (varn_name "x")]) ``;
+
 
 val test_NEWFRAME2 =
-prove(`` e_red    (^ctx9)(^prog_call6a) 
-                  (^stacks_call6a) (^R)
-                  (e_func_exec stmt_empty) 
-                  (^stacks_call6b) (^R)``,
+prove(`` e_red (^ctx8) ^scope2 [FEMPTY]
+                  (^prog_call13) 
+                  (e_var varn_star) [("Add1", stmt_empty , [^scope14] )]``,
 
-RW.ONCE_RW_TAC[e_red_cases] >>
-EVAL_TAC>>
-
-DISJ2_TAC >> DISJ1_TAC >>
-EXISTS_TAC ``[( (e_var "x")
+EXP_SIMP >>
+EXISTS_TAC ``[( (e_var (varn_name "x"))
 	       , "y"
-	       , d_out)]`` >>
-	       
-REPEAT (EVAL_TAC>>
-FULL_SIMP_TAC list_ss [] )
-
+	       , d_out)]`` >>	       	       
+EVAL_TAC>>
+FULL_SIMP_TAC list_ss []
 );
 
 
 
 (****copy_in two args IN and OUT values aka func_call_newframe rule ****)
-val stacks_call7a  = ``(stacks_tup ^scopelist14 [])``;
-val stacks_call7b  = ``(stacks_tup ^scopelist21 [([] , ^Fn "Add1")])``;
-
+(* test 10: copy_in two arguments (NONE, OUT) values aka func_call_newframe rule*)
 val ctx9 = ``(FEMPTY, ^func_sig4, FEMPTY, FEMPTY, empty_ctrl):ctx``;
 
 val test_NEWFRAME3 =
-prove(`` e_red    (^ctx9)(^prog_call3b) 
-                  (^stacks_call7a) (^R)
-                  (e_func_exec stmt_empty) 
-                  (^stacks_call7b) (^R)``,
-RW.ONCE_RW_TAC[e_red_cases] >>
-EVAL_TAC>>
-FULL_SIMP_TAC list_ss [] >>
+prove(`` e_red (^ctx4) ^scope0 [^scope8]
+                  (^prog_call6) 
+                   (e_var varn_star) [("Add1", stmt_empty , [^scope15] )] ``,
+		  
+EXP_SIMP >>
 EXISTS_TAC ``[( (e_v (v_bit ([F],1))) , "a" , d_none);
-              (  e_var"y"          , "b" , d_out)]`` >>
+              ( e_var ( varn_name "y"), "b" , d_out)]`` >>      
 EVAL_TAC
 );
-
-
-
-
-(*call a function from an other function*)
-(*
-val func_sig9 = ``(FEMPTY |+ ("Add1",(stmt_ass lval_null (e_func_call "Sub" [e_var "x"])) , [("a",d_in)] ))
-                          |+ ("Sub" ,(stmt_empty , [("b",d_none)]))``;
-
-val ctx10 = ``(FEMPTY, ^func_sig9, FEMPTY, FEMPTY, empty_ctrl):ctx``;
-
-val prog_call7a= ``e_func_exec (stmt_ass lval_null (e_func_call "Sub" [e_var "x"]))``;
-val prog_call7b= ``e_func_exec (stmt_ass lval_null (e_func_call "Sub" [e_v (v_bit ([F],1))]))``;
-val prog_call7c= ``e_func_exec (stmt_ass lval_null (e_func_exec  stmt_empty))``;
-
-val stacks_call8a  = ``(stacks_tup ^scopelist23 [([] , ^Fn "Add1")])``;
-
-
-val test_NEWFRAME4 =
-prove(`` e_red    (^ctx10)(^prog_call7a) 
-                  (^stacks_call8a) (^R)
-                  (^prog_call7b) 
-                  (^stacks_call8a) (^R)``,
-
-RW.ONCE_RW_TAC[e_red_cases] >>
-EVAL_TAC>>
-FULL_SIMP_TAC list_ss [] >>
-*)
-
-
-
 
 
 
 (**************************************************************)
 (*** Testing apply and tables reductions --concrete values-- ***)
 (**************************************************************)
-val prog_stmt_apply1 = ``stmt_app "check_ttl" (e_var ("headers.ip.ttl")) ``;
-val prog_stmt_apply2 = ``stmt_app "check_ttl" (e_v (v_bit ([T; F],2))) ``;
-val prog_stmt_apply3 = ``stmt_ass lval_null   (e_func_call "NoAction" [])``;
+val prog_app1 = ``stmt_app "check_ttl" (e_var (varn_name("headers.ip.ttl"))) ``;
+val prog_app2 = ``stmt_app "check_ttl" (e_v (v_bit ([T; F],2))) ``;
+val prog_app3 = ``stmt_ass lval_null   (e_func_call "NoAction" [])``;
 
-val state13a = ``state_tup (stacks_tup (^scopelist22) []) ^R``;
-
-val table_map1 = ``(FEMPTY |+ ("check_ttl", (e_var("headers.ip.ttl") , match_kind_exact)))``;
+val table_map1 = ``(FEMPTY |+ ("check_ttl", (e_var(varn_name ("headers.ip.ttl")) , match_kind_exact)))``;
 
 val ctrl1 = Define
 `
  ctrl1 (("check_ttl"), (v_bit ([F; F],2)), (match_kind_exact)) = SOME ("Send_to_cpu",[]:e list ) /\
- ctrl1 (("check_ttl"),          x        , (match_kind_exact)) = SOME ("NoAction",[]:e list )
+ ctrl1 (("check_ttl"), (v_bit ([T; F],2)) , (match_kind_exact)) = SOME ("NoAction",[]:e list )
 `;
+
 val ctx11 = ``(FEMPTY, FEMPTY, FEMPTY, ^table_map1, ctrl1):ctx``;
 
 
-val test_TABLE1 =
+(* test 1: test two reductions app e -> app v -> null := call f     *)
+
+val frame_app1 = `` [("f", ^prog_app1 , ^scopelist4 )] : Frame_list `` ;
+val state_app1 = ``(state_P4 ^scope16 (^frame_app1) ^R): state``;
+
+val frame_app2 = `` [("f", ^prog_app2 , ^scopelist4 )] : Frame_list `` ;
+val state_app2 = ``(state_P4 ^scope16 (^frame_app2) ^R): state``;
+
+val frame_app3 = `` [("f", ^prog_app3 , ^scopelist4 )] : Frame_list `` ;
+val state_app3 = ``(state_P4 ^scope16 (^frame_app3) ^R): state``;
+
+
+val test_APPLY1 =
 prove(``
-(stmt_red (^ctx11)(^prog_stmt_apply1) 
-                  (^state13a) 
-                  (^prog_stmt_apply2) 
-                  (^state13a)) /\
+(stmt_red ^ctx11 ^state_app1 ^state_app2) /\
+(stmt_red ^ctx11 ^state_app2 ^state_app3)  ``,
 
-
-(stmt_red (^ctx11)(^prog_stmt_apply2) 
-                  (^state13a) 
-                  (^prog_stmt_apply3) 
-                  (^state13a)) ``,
-
-NTAC 2 (RW.ONCE_RW_TAC[e_red_cases] >>
-EVAL_TAC>>
-FULL_SIMP_TAC list_ss []) >>
+CONJ_TAC >|[
+STMT_SIMP>>
+EXP_SIMP>>
 EVAL_TAC
-);
+,
+NTAC 2 (RW.ONCE_RW_TAC[stmt_red_cases] >>
+EVAL_TAC>>
+FULL_SIMP_TAC list_ss [ctrl1])
+]);
 
 
 
 
+(* test 2: test two reductions app e -> app v -> null := call f
+Where teh value is repeated in teh global and in the local stack scope *)
 
-val prog_stmt_apply2b = ``stmt_app "check_ttl" (e_v (v_bit ([F],1))) ``;
-val prog_stmt_apply3b = ``stmt_ass lval_null   (e_func_call "Send_to_cpu" [])``;
-val state13b = ``state_tup (stacks_tup (^scopelist24) []) ^R``;
+val prog_app4 = ``stmt_app "check_ttl" (e_v (v_bit ([F],1))) ``;
+val prog_app5 = ``stmt_ass lval_null   (e_func_call "Send_to_cpu" [])``;
+
+val frame_app4 = `` [("f", ^prog_app1 , ^scopelist24 )] : Frame_list `` ;
+val state_app4 = ``(state_P4 ^scope16 (^frame_app4) ^R): state``;
+
+val frame_app5 = `` [("f", ^prog_app4 , ^scopelist24 )] : Frame_list `` ;
+val state_app5 = ``(state_P4 ^scope16 (^frame_app5) ^R): state``;
+
+val frame_app6 = `` [("f", ^prog_app5 , ^scopelist24 )] : Frame_list `` ;
+val state_app6 = ``(state_P4 ^scope16 (^frame_app6) ^R): state``;
+
 
 val ctrl2 = Define
 `
  ctrl2 (("check_ttl"), (v_bit ([F],1)), (match_kind_exact)) = SOME ("Send_to_cpu",[]:e list ) /\
- ctrl2 (("check_ttl"),        x       , (match_kind_exact)) = SOME ("NoAction"   ,[]:e list )
+ ctrl2 (("check_ttl"), (v_bit ([],1)), (match_kind_exact)) = SOME ("NoAction"   ,[]:e list )
 `;
 
+(*
+val x = Define `
+f (1,5) = 0 /\
+f (1,x) = 1
+`
+*)
 
 val ctx12 = ``(FEMPTY, FEMPTY, FEMPTY, ^table_map1, ctrl2):ctx``;
 
-val test_TABLE2 =
+val test_APPLY2 =
 prove(``
-(stmt_red (^ctx12)(^prog_stmt_apply1) 
-                  (^state13b) 
-                  (^prog_stmt_apply2b) 
-                  (^state13b))   /\
-		  
-(stmt_red (^ctx12)(^prog_stmt_apply2b) 
-                  (^state13b) 
-                  (^prog_stmt_apply3b) 
-                  (^state13b)) ``,
+(stmt_red ^ctx12 ^state_app4 ^state_app5) /\
+(stmt_red ^ctx12 ^state_app5 ^state_app6) ``,
 
-NTAC 2 (RW.ONCE_RW_TAC[e_red_cases] >>
-EVAL_TAC>>
-FULL_SIMP_TAC list_ss []) >>
+CONJ_TAC >|[
+STMT_SIMP>>
+EXP_SIMP>>
 EVAL_TAC
-);
+,
+NTAC 2 (RW.ONCE_RW_TAC[stmt_red_cases] >>
+EVAL_TAC>>
+FULL_SIMP_TAC list_ss [ctrl2])
+]);
 
 
 
@@ -1050,107 +968,140 @@ EVAL_TAC
 (***    Testing return reductions --concrete values--       ***)
 (**************************************************************)
 
-
-
+(*test a value assigned to a function call... with a copy out
+and the body of teh funtion is return *)
 
 val func_sig10 = ``(FEMPTY |+ ("Add1", (stmt_ret (e_v (v_bit ([F;F],2))) , [("y",d_out)] )))``;
-val ctx9 = ``(FEMPTY, ^func_sig10, FEMPTY, FEMPTY, empty_ctrl):ctx``;
-val prog_call9a = ``(e_func_call "Add1" [e_var "x"]) ``;
-val prog_call9b = ``(e_func_exec (stmt_ret (e_v (v_bit ([F;F],2))))) ``;
+val ctx13 = ``(FEMPTY, ^func_sig10, FEMPTY, FEMPTY, empty_ctrl):ctx``;
 
-val prog_return1a = ``((stmt_ret (e_v (v_bit ([F;F],2))))) ``;
-val prog_return1b = ``(stmt_empty)``;
+val prog_ret1 = ``(stmt_ass (lval_varname (varn_name"g")) (e_func_call "Add1" [e_var (varn_name "x")]))  ``;
+val prog_ret2a = ``(stmt_ret (e_v (v_bit ([F;F],2)))) ``;
+val prog_ret2b = ``(stmt_ass (lval_varname (varn_name"g"))  (e_var varn_star))  ``;
 
-val prog_return2a = ``(e_func_exec (stmt_ret (e_v (v_bit ([F;F],2))))) ``;
-val prog_return2b = ``(e_func_exec stmt_empty) ``;
+val frame_ret1 = `` [("f", ^prog_ret1 , ^scopelist17 )] : Frame_list `` ;
+val state_ret1 = ``(state_P4 FEMPTY (^frame_ret1) ^R): state``;
 
-val stacks_call9a  = ``(stacks_tup ^scopelist17 [])``;
-val stacks_call9b  = ``(stacks_tup ^scopelist25 [([] , ^Fn "Add1")])``;
+val frame_ret2a = `` [("Add1", ^prog_ret2a , ^scopelist26 )] : Frame_list `` ;
+val frame_ret2b = `` [("f", ^prog_ret2b , ^scopelist17 )] : Frame_list `` ;
 
-
-
-val state14a = ``(state_tup (stacks_tup ^scopelist25 [([] , ^Fn "Add1")]) ^R): state``;
-val state14b = ``(state_tup (stacks_tup ^scopelist17 [])
-                       (status_return  (v_bit ([F;F],2)))):state``;
+val state_ret2 = ``(state_P4 FEMPTY ((^frame_ret2a)++(^frame_ret2b)) ^R): state``;
 
 
-
+(* test 1:
+test reduction [f, g := call Add1 (x), oldf] -> [Add1, ret 0 , cpins]++[ f, g := * , oldf]
+*)
 
 val test_return1 =
-prove(`` (e_red   (^ctx9)(^prog_call9a) 
-                  (^stacks_call9a) (^R)
-                  (^prog_call9b) 
-                  (^stacks_call9b) (^R))
-
-     /\  (e_red    (^ctx9)(^prog_return2a) 
-                  (^stacks_call9b) (^R)
-                  (^prog_return2b) 
-                  (^stacks_call9a) ((status_return  (v_bit ([F;F],2)))))
-
-
-
+prove(`` stmt_red ^ctx13 ^state_ret1 ^state_ret2
 ``,
-CONJ_TAC >| [
-RW.ONCE_RW_TAC[e_red_cases] >>
-EVAL_TAC>>
-DISJ2_TAC >> DISJ1_TAC >>
-EXISTS_TAC ``[( (e_var "x")
+
+STMT_SIMP >>
+EXISTS_TAC``^frame_ret2a`` >>
+EXISTS_TAC``  (e_var varn_star)``>>
+EXP_SIMP >>
+EXISTS_TAC ``[( e_var (varn_name "x")
 	       , "y"
 	       , d_out)]`` >>	       
-REPEAT (EVAL_TAC>>
-FULL_SIMP_TAC list_ss [] )
-,
-REPEAT(RW.ONCE_RW_TAC[e_red_cases] >>
 EVAL_TAC>>
-FULL_SIMP_TAC list_ss [FUPDATE_EQ]) 
-]
+FULL_SIMP_TAC list_ss []
 );
 
 
 
 
+(* test 2:
+test reduction [Add1, ret 0 , cpins] ++ [ f, g := * , oldf] -> [f, g = * , oldf']
+with copyouts
+*)
 
-val prog_return2a = ``(e_func_exec (stmt_ret (e_v (v_bit ([F;F],2))))) ``;
-val prog_return2b = ``(e_func_exec stmt_empty) ``;
+val frame_ret2a = `` [("Add1", ^prog_ret2a , ^scopelist26 )] : Frame_list `` ;
+val frame_ret2b = `` [("f", ^prog_ret2b , ^scopelist28 )] : Frame_list `` ;
+
+val state_ret2 = ``(state_P4 FEMPTY ((^frame_ret2a)++(^frame_ret2b)) ^R): state``;
+
+
+val frame_ret3a = `` [("Add1", stmt_empty , ^scopelist26 )] : Frame_list `` ;
+val frame_ret3b = `` [("f", ^prog_ret2b , ^scopelist27 )] : Frame_list `` ; (*same as 2a*)
+val state_ret3 = ``(state_P4 FEMPTY ((^frame_ret3b)) ^R ) : state``;
+
 
 val test_return2 =
-prove(`` (stmt_red (^ctx9)(^prog_return1a) 
-                  (^state14a)
-                  (^prog_return1b) 
-                  (^state14b))
+prove(`` stmt_red ^ctx13 ^state_ret2 ^state_ret3 
 ``,
+FULL_SIMP_TAC list_ss [Once stmt_red_cases ] >>
+DISJ2_TAC >> DISJ1_TAC >>
 
-RW.ONCE_RW_TAC[e_red_cases] >>
-DISJ1_TAC >>
-EVAL_TAC>>
-EXISTS_TAC ``[(  "y", d_out)]`` >>	       
-EVAL_TAC>>
-FULL_SIMP_TAC list_ss [] >>
+
+EXISTS_TAC `` [("y",d_out)]`` >>
+EXISTS_TAC ``FEMPTY : scope`` >>
 EXISTS_TAC ``"Add1"`` >>
 EXISTS_TAC ``stmt_ret (e_v (v_bit ([F; F],2)))`` >>
-EVAL_TAC>>
-FULL_SIMP_TAC list_ss [FUPDATE_EQ]
+EXISTS_TAC ``[FEMPTY |+ (varn_name "y",v_bit ([F],1),SOME (lval_varname (varn_name "x")))]`` >>
+
+EXISTS_TAC ``"f"`` >>
+EXISTS_TAC ``stmt_ass (lval_varname (varn_name "g")) (e_var varn_star)`` >>
+EXISTS_TAC ``^scopelist28`` >>
+EXISTS_TAC ``[] : Frame_list`` >>
+EXISTS_TAC ``FEMPTY : scope`` >>
+EXISTS_TAC ``^scopelist27`` >>
+
+EXISTS_TAC ``stmt_empty`` >>
+EXISTS_TAC ``(v_bit ([F; F],2))`` >>
+
+EXISTS_TAC ``stmt_ret (e_v (v_bit ([F; F],2)))`` >>
+
+STMT_SIMP >>
+
+
+ASSUME_TAC (finite_mapLib.fupdate_NORMALISE_CONV
+``FEMPTY |+ ("y",v_bit ([T],1),NONE) |+ ("x",v_bit ([F],1),NONE) |+
+   ("star",v_bit ([F; F],2),NONE) |+ ("x",v_bit ([F],1),NONE)``) >>
+fs [FUPDATE_COMMUTES]
 );
 
 
 
 
-val prog_return2b = ``(e_func_exec stmt_empty) ``;
-val prog_return2c = ``(e_v (v_bit ([F;F],2))) ``;
+(* test 3:
+test reduction [Add1, ret 0 , cpins] ++ [ f, g := * , oldf] -> [f, g = * , oldf']
+without copyouts
+*)
 
-val stacks_call_ret1 = ``(stacks_tup ^scopelist17 [])``;
+val frame_ret4a = `` [("Add1", ^prog_ret2a , [FEMPTY] )] : Frame_list `` ;
+val frame_ret4b = `` [("f", ^prog_ret2b , ^scopelist28 )] : Frame_list `` ;
+val state_ret4 = ``(state_P4 FEMPTY ((^frame_ret4a)++(^frame_ret4b)) ^R): state``;
+
+val frame_ret5b = `` [("f", ^prog_ret2b , ^scopelist27 )] : Frame_list `` ; 
+val state_ret5 = ``(state_P4 FEMPTY ((^frame_ret5b)) ^R ) : state``;
+
 
 val test_return3 =
-prove(`` e_red (^ctx9)(^prog_return2b) 
-                (^stacks_call_ret1) (status_return  ((v_bit ([F;F],2))))
-                (^prog_return2c) 
-                (^stacks_call_ret1) (^R)
+prove(`` stmt_red ^ctx7 ^state_ret4 ^state_ret5 
 ``,
+FULL_SIMP_TAC list_ss [Once stmt_red_cases ] >>
+DISJ2_TAC >> DISJ1_TAC >>
 
-RW.ONCE_RW_TAC[e_red_cases] >>
-NTAC 3 DISJ2_TAC >> DISJ1_TAC >>
-EXISTS_TAC ``v_bit ([F; F],2)`` >>
-EVAL_TAC
+
+EXISTS_TAC `` [("y",d_in)]`` >>
+EXISTS_TAC ``FEMPTY : scope`` >>
+EXISTS_TAC ``"Add1"`` >>
+EXISTS_TAC ``stmt_ret (e_v (v_bit ([F; F],2)))`` >>
+EXISTS_TAC ``[FEMPTY]:scopes_stack`` >>
+
+EXISTS_TAC ``"f"`` >>
+EXISTS_TAC ``stmt_ass (lval_varname (varn_name "g")) (e_var varn_star)`` >>
+EXISTS_TAC ``^scopelist28`` >>
+EXISTS_TAC ``[] : Frame_list`` >>
+EXISTS_TAC ``FEMPTY : scope`` >>
+EXISTS_TAC ``^scopelist27`` >>
+
+
+EXISTS_TAC ``stmt_empty`` >>
+EXISTS_TAC ``(v_bit ([F; F],2))`` >>
+EXISTS_TAC ``stmt_empty`` >>
+
+STMT_SIMP>>
+FULL_SIMP_TAC list_ss [FLOOKUP_DEF, LUPDATE_def, FUPDATE_EQ]
 );
 
 
@@ -1171,36 +1122,41 @@ val header2 = `` [("dstAddr", (v_bit ([T;T],2)));
 		 ``;
 
 
-val scopelist_h1 = ``[FEMPTY |+ ("IPv4_h",((v_header (T) ^header1) , NONE:string option))]``;
+val scopelist_h1 = ``[FEMPTY |+ (varn_name "IPv4_h",((v_header (T) ^header1) , NONE:lval option))] ``;
 
-val scopelist_h2 = ``[FEMPTY |+ ("IPv4_h",((v_header (T) ^header2) , NONE:string option))]``;
-
-
-val state15a = ``(state_tup (stacks_tup ^scopelist_h1 []) ^R):state``;
+val scopelist_h2 = ``[FEMPTY |+ (varn_name "IPv4_h",((v_header (T) ^header2) , NONE:lval option))]``;
 
 
-val prog_ass_h1a = ``stmt_ass  (lval_field (lval_varname "IPv4_h") "srcAddr")
+val prog_ass_h1 = ``stmt_ass  (lval_field (lval_varname (varn_name "IPv4_h")) "srcAddr")
                                   (e_v (v_bit ([T;T],2)))``;
 
-val prog_ass_h1b = ``stmt_ass  ( (lval_varname "IPv4_h"))
+val prog_ass_h2 = ``stmt_ass  (lval_varname (varn_name "IPv4_h"))
                                   (e_v (v_header (T) ^header2)) ``;
 
 
+val frame_ass_h1 = `` [("f", ^prog_ass_h1 , ^scopelist_h1 )] : Frame_list `` ;
+val state_ass_h1 = ``(state_P4 FEMPTY (^frame_ass_h1) ^R): state``;
+
+val frame_ass_h2 = `` [("f", stmt_empty , ^scopelist_h2 )] : Frame_list `` ;
+val state_ass_h2 = ``(state_P4 FEMPTY (^frame_ass_h2) ^R): state``;
+
+
+(* test 1: test assigning a value to a header feild *)
 
 val test_ass_h1 =
-prove(`` (stmt_red (^ctx_empty)(^prog_ass_h1a) 
-                  (^state15a)
-                  (^prog_ass_h1b) 
-                  (^state15a))
+prove(`` stmt_red ^ctx_empty ^state_ass_h1 ^state_ass_h2
 ``,
-RW.ONCE_RW_TAC[e_red_cases] >>
-EVAL_TAC>>
-FULL_SIMP_TAC std_ss []>>
-DISJ2_TAC>>
-NTAC 2 (EVAL_TAC>>
-SIMP_TAC std_ss [])
+STMT_SIMP >>
+DISJ1_TAC >>
+FULL_SIMP_TAC std_ss [] >>
+EVAL_TAC >>
+FULL_SIMP_TAC list_ss [FUPDATE_EQ]
 );
 
+
+
+
+(* test 2: test assigning a whole header to a header feild *)
 
 val header3 = `` [("dstAddr", (v_bit ([F;F],2)));
                  ("srcAddr", (v_bit ([F;F],2)));
@@ -1208,29 +1164,30 @@ val header3 = `` [("dstAddr", (v_bit ([F;F],2)));
 		 ``;
 
 
-val scopelist_h3 = ``[FEMPTY |+ ("IPv4_h",((v_header (T) ^header3) , NONE:string option))]``;
+val scopelist_h3 = ``[FEMPTY |+ (varn_name "IPv4_h",((v_header (T) ^header3) , NONE:lval option))]``;
 
 
-val prog_ass_h1c = ``stmt_ass  (lval_field (lval_varname "IPv4_h") "dstAddr")
-                                  (e_v (v_bit ([F;F],2)))``;
-
-val prog_ass_h1d = ``stmt_ass  ( (lval_varname "IPv4_h"))
-                                  (e_v (v_header (T) ^header3)) ``;
+val prog_ass_h3 = ``stmt_ass  (lval_varname (varn_name "IPv4_h"))
+                                (e_v (v_header (T) ^header3))``;
 
 
 
-val test_ass_h2 =
-prove(`` (stmt_red (^ctx_empty)(^prog_ass_h1c) 
-                  (^state15a)
-                  (^prog_ass_h1d) 
-                  (^state15a))
+val frame_ass_h3 = `` [("f", ^prog_ass_h3 , ^scopelist_h2 )] : Frame_list `` ;
+val state_ass_h3 = ``(state_P4 FEMPTY (^frame_ass_h3) ^R): state``;
+
+
+val frame_ass_h4 = `` [("f", stmt_empty , ^scopelist_h3 )] : Frame_list `` ;
+val state_ass_h4 = ``(state_P4 FEMPTY (^frame_ass_h4) ^R): state``;
+
+
+val test_ass_h3 =
+prove(`` stmt_red (^ctx_empty) ^state_ass_h3 ^state_ass_h4
 ``,
-RW.ONCE_RW_TAC[e_red_cases] >>
-EVAL_TAC>>
-FULL_SIMP_TAC std_ss []>>
-DISJ2_TAC>>
-NTAC 2 (EVAL_TAC>>
-SIMP_TAC std_ss [])
+STMT_SIMP >>
+DISJ1_TAC >>
+FULL_SIMP_TAC std_ss [] >>
+EVAL_TAC >>
+FULL_SIMP_TAC list_ss [FUPDATE_EQ]
 );
 
 
@@ -1239,21 +1196,18 @@ SIMP_TAC std_ss [])
 
 (*access fields*)
 
-val prog_acc_h1a = ``e_acc (e_v (v_header (T) (^header1))) (e_var("srcAddr"))  ``;
-val prog_acc_h1b = ``e_v  (v_bit ([F; F],2)) ``;
-val stacks_h1    = ``(stacks_tup ^scopelist_h1 [])``;
+val prog_acc_h1 = ``e_acc (e_v (v_header (T) (^header1))) (e_v( v_str "srcAddr"))  ``;
+val prog_acc_h2 = ``e_v  (v_bit ([F; F],2)) ``;
 
 
 val test_acc_h1 =
-prove(`` (e_red  (^ctx_empty)(^prog_acc_h1a) 
-                  (^stacks_h1) ^R
-                  (^prog_acc_h1b) 
-                  (^stacks_h1) ^R)
+prove(`` e_red (^ctx_empty) FEMPTY ^scopelist_h1
+               (^prog_acc_h1) (^prog_acc_h2) ([])
 ``,
-RW.ONCE_RW_TAC[e_red_cases] >>
-NTAC 2 (EVAL_TAC>>
-FULL_SIMP_TAC std_ss [])
+REPEAT EXP_SIMP
 );
+
+
 
 
 
@@ -1273,59 +1227,1027 @@ val struct2 = ``[("Ethernet_h", (v_bit ([F;F],2)));
                  ("IPv4_h", (v_header (T) ^header1))]``;
 
 
-val scopelist_s1 =``[FEMPTY |+ ("Parsed_packet", ((v_struct ^struct1), NONE:string option))]``;
-val scopelist_s2 =``[FEMPTY |+ ("Parsed_packet", ((v_struct ^struct2), NONE:string option))]``;
+val scopelist_s1 =``[FEMPTY |+ (varn_name "Parsed_packet", ((v_struct ^struct1), NONE:lval option))]``;
+val scopelist_s2 =``[FEMPTY |+ (varn_name "Parsed_packet", ((v_struct ^struct2), NONE:lval option))]``;
 
-val prog_ass_s1a = ``stmt_ass  (lval_field (lval_varname "Parsed_packet") "Ethernet_h")
+val prog_ass_s1 = ``stmt_ass  (lval_field (lval_varname (varn_name "Parsed_packet")) "Ethernet_h")
                                   (e_v (v_bit ([F;F],2)))``;
 
-val prog_ass_s1b = ``stmt_ass  ( (lval_varname "Parsed_packet"))
-                                  (e_v (v_struct ^struct2)) ``;
 
+val frame_ass_s1 = `` [("f", ^prog_ass_s1 , ^scopelist_s1 )] : Frame_list `` ;
+val state_ass_s1 = ``(state_P4 FEMPTY (^frame_ass_s1) ^R): state``;
 
-val state16a = ``(state_tup (stacks_tup ^scopelist_s1 []) ^R):state``;
-val state16b = ``(state_tup (stacks_tup ^scopelist_s2 []) ^R):state``;
+val frame_ass_s2 = `` [("f", stmt_empty , ^scopelist_s2 )] : Frame_list `` ;
+val state_ass_s2 = ``(state_P4 FEMPTY (^frame_ass_s2) ^R): state``;
+
 
 val test_ass_s1 =
-prove(`` (stmt_red (^ctx_empty)(^prog_ass_s1a) 
-                  (^state16a)
-                  (^prog_ass_s1b) 
-                  (^state16a))  /\
-		  
-         (stmt_red (^ctx_empty)(^prog_ass_s1b) 
-                  (^state16a)
-                  (stmt_empty) 
-                  (^state16b))		  
-         		  
+prove(`` stmt_red ^ctx_empty ^state_ass_s1 ^state_ass_s2       		  
+``,
+STMT_SIMP >>
+DISJ1_TAC >>
+FULL_SIMP_TAC std_ss [] >>
+EVAL_TAC >>
+FULL_SIMP_TAC list_ss [FUPDATE_EQ]
+);
+
+
+val prog_acc_h1 = ``e_acc (e_v (v_header (T) (^header1))) (e_v( v_str "srcAddr"))  ``;
+val prog_acc_h2 = ``e_v  (v_bit ([F; F],2)) ``;
+
+
+val prog_acc_s1 = ``e_acc (e_v (v_struct (^struct1))) (e_v( v_str "IPv4_h"))  ``;
+val prog_acc_s2 = ``e_v  (v_header (T) (^header1) ) ``;
+
+
+val test_acc_h1 =
+prove(`` e_red  (^ctx_empty) FEMPTY ^scopelist_s1
+                  ^prog_acc_s1 ^prog_acc_s2 ([])
+``,
+NTAC 2 EXP_SIMP
+);
+
+
+(****************************************************************)
+(***          Testing A block calling a function              ***)
+(****************************************************************)
+
+
+(*
+
+JR (out y)    //Just Return function
+{
+Return ((e_v (v_bit ([F;F],2));
+}
+
+
+
+f()
+{
+  {
+    <--- start from here
+    g := call JR (x)
+  }
+}
+
+*)
+
+(*
+
+val func_sig11 = ``(FEMPTY |+ ("JR", (stmt_ret (e_v (v_bit ([F;F],2))) , [("y",d_out)] )))``;
+val ctx13 = ``(FEMPTY, ^func_sig11, FEMPTY, FEMPTY, empty_ctrl):ctx``;
+
+val prog_test1 = ``(stmt_ass (lval_varname "g") (e_func_call "JR" [e_var "x"]))  ``;
+
+val prog_test2a = ``(stmt_ret (e_v (v_bit ([F;F],2)))) ``;
+val prog_test2b = ``(stmt_ass (lval_varname "g") (e_var "star") ) ``;
+
+val frame_test1 = `` [("f", ^prog_ret1 , ^scopelist17 )] : Frame_list `` ;
+val state_test1 = ``(state_P4 FEMPTY (^frame_ret1) ^R): state``;
+
+
+
+val frame_ret2a = `` [("JR", ^prog_ret2a , ^scopelist26 )] : Frame_list `` ;
+val frame_ret2b = `` [("f", ^prog_ret2b , ^scopelist17 )] : Frame_list `` ;
+
+val state_ret2 = ``(state_P4 FEMPTY ((^frame_ret2a)++(^frame_ret2b)) ^R): state``;
+
+
+(* test 1:
+test reduction [f, g := call Add1 (x), oldf] -> [Add1, ret 0 , cpins]++[ f, g := * , oldf]
+*)
+
+val test_return1 =
+prove(`` stmt_red ^ctx13 ^state_ret1 ^state_ret2
 ``,
 
-CONJ_TAC>| [
-NTAC 3 (
-RW.ONCE_RW_TAC[e_red_cases] >>
+STMT_SIMP >>
+EXISTS_TAC``^frame_ret2a`` >>
+EXISTS_TAC`` (e_var "star")``>>
+EXP_SIMP >>
+EXISTS_TAC ``[( (e_var "x")
+	       , "y"
+	       , d_out)]`` >>
+EXISTS_TAC ``^scopelist17`` >>	       
 EVAL_TAC>>
-FULL_SIMP_TAC std_ss [])
+FULL_SIMP_TAC list_ss []
+);
+
+*)
+
+
+(******************************************)
+(******************************************)
+(******************************************)
+(******************************************)
+(******************************************)
+(******************************************)
+(******************************************)
+(******************************************)
+(******************************************)
+(******************************************)
+(******************************************)
+(******************************************)
+
+(******** SAME SATE and EXP DEF ************)
+(*********Mapping equv. lemmas ************)
+
+
+open ottTheory;
+open pairTheory;
+open rich_listTheory;
+
+val lemma_MAP1 =
+prove(``
+! (l1: (e#string#d) list) l2 . ( MAP (λ(e_,x_,d_). (x_,d_)) l1 ) = ( MAP (λ(e_,x_,d_). (x_,d_)) l2 ) ==>
+(? (le1 : e list)  (lx1 : string list)  (ld1 : d list) (le2 : e list) lx2 ld2.
+ MAP (λ(e_,x_,d_). (x_,d_)) (ZIP (le1, ZIP(lx1, ld1))) =
+ MAP (λ(e_,x_,d_). (x_,d_)) (ZIP (le2, ZIP(lx2, ld2)))  /\ le1 = le2 /\ lx1 = lx2 /\ ld1 = ld2 ) ``,
+
+REPEAT STRIP_TAC >>
+NTAC 2 (EXISTS_TAC``[]: e list`` >>
+EXISTS_TAC``[]: x list`` >>
+EXISTS_TAC``[]: d list`` ) >>
+FULL_SIMP_TAC list_ss []
+);
+
+val lemma_MAP2 =
+prove (``!l. MAP (λ(e_,x_,d_). (x_,d_)) l = MAP SND l``,
+
+Induct_on `l` >>
+FULL_SIMP_TAC list_ss [] >>
+STRIP_TAC >>
+Cases_on `h` >>
+Cases_on `r` >>
+FULL_SIMP_TAC list_ss [] 
+);
+
+val lemma_MAP3 =
+prove(`` !(l: (e#string#d) list) l' . (MAP (λ(e_ : e ,x_,d_). (x_,d_)) l = MAP (λ(e_,x_,d_). (x_,d_)) l') ==>
+MAP SND l = MAP SND l'``,
+FULL_SIMP_TAC list_ss [lemma_MAP2] 
+);
+
+val lemma_MAP4 =
+prove(`` !(l: (e#string#d) list) l' . (MAP (λ(e_ : e ,x_,d_). (x_,d_)) l = MAP (λ(e_,x_,d_). (x_,d_)) l') /\
+(MAP FST l = MAP FST l') ==>
+(l = l')  ``,
+FULL_SIMP_TAC list_ss [lemma_MAP2, lemma_MAP1, lemma_MAP3] >>
+RW_TAC list_ss [PAIR_FST_SND_EQ,LIST_EQ_MAP_PAIR] 
+
+);
+
+
+
+val lemma_MAP5 =
+prove (``!(l: (e#string#d) list) (l': (e#e#string#d) list)  .
+          (MAP (λ(e_,x_,d_). (x_,d_)) l =
+        MAP (λ(e_,e'_,x_,d_). (x_,d_)) l') ==> 
+        ((MAP (λ(e_,x_,d_). d_) l) = (MAP (λ(e_,e'_,x_,d_). d_) l')) /\
+        ((MAP (λ(e_,x_,d_). x_) l) = (MAP (λ(e_,e'_,x_,d_). x_) l'))``,
+
+
+Induct_on `l` >>
+Induct_on `l'` >>
+FULL_SIMP_TAC list_ss [] >>
+NTAC 3 STRIP_TAC>>
+
+Cases_on `h` >>
+Cases_on `h'` >>
+Cases_on `r` >>
+Cases_on `r'` >>
+Cases_on `r''` >>
+REV_FULL_SIMP_TAC list_ss []
+);
+
+
+
+val lemma_MAP6 =
+prove (``
+!(e_e'_x_d_list: (e#e#string#d) list) (e_e'_x_d_list': (e#e#string#d) list) .
+        (MAP (λ(e_,e'_,x_,d_). (x_,d_)) e_e'_x_d_list =
+        MAP (λ(e_,e'_,x_,d_). (x_,d_)) e_e'_x_d_list') ==>
+	(MAP (λ(e_,e'_,x_,d_). d_) e_e'_x_d_list =
+        MAP (λ(e_,e'_,x_,d_). d_) e_e'_x_d_list') ``,
+
+Induct_on `e_e'_x_d_list` >>
+Induct_on `e_e'_x_d_list'` >>
+FULL_SIMP_TAC list_ss [] >>
+NTAC 3 STRIP_TAC>>
+
+Cases_on `h` >>
+Cases_on `h'` >>
+Cases_on `r` >>
+Cases_on `r'` >>
+Cases_on `r` >>
+Cases_on `r''` >>
+REV_FULL_SIMP_TAC list_ss []
+);
+
+
+
+
+
+
+val lemma_MAP7 =
+prove ( ``
+!(e_x_d_list: (e#string#d) list) (e_x_d_list': (e#string#d) list) .
+        (MAP (λ(e_,x_,d_). (x_,d_)) e_x_d_list =
+        MAP (λ(e_,x_,d_). (x_,d_)) e_x_d_list') ==>
+	(MAP (λ(e_,x_,d_). (x_)) e_x_d_list =
+        MAP (λ(e_,x_,d_). (x_)) e_x_d_list') /\
+	(MAP (λ(e_,x_,d_). (d_)) e_x_d_list =
+        MAP (λ(e_,x_,d_). (d_)) e_x_d_list') ``,
+
+Induct_on `e_x_d_list` >>
+Induct_on `e_x_d_list'` >>
+FULL_SIMP_TAC list_ss [] >>
+NTAC 3 STRIP_TAC>>
+
+Cases_on `h` >>
+Cases_on `h'` >>
+Cases_on `r` >>
+Cases_on `r'` >>
+REV_FULL_SIMP_TAC list_ss []
+);
+
+
+
+
+(********* lval and is_const lemmas ************)
+
+val lemma_const_notlval =
+prove (``!e. is_const e ==> ~ is_e_lval e``,
+Cases_on `e` >>
+EVAL_TAC
+);
+
+val lemma_lval_notconst =
+prove (``!e. is_e_lval e ==> ~ is_const e``,
+Cases_on `e` >>
+EVAL_TAC
+);
+
+
+(********* Proving the mono P Q  lemmas ************)
+
+(**************************
+P is (is_d_none_in d ∧ ¬is_const e)
+Q is ((is_d_none_in d ⇒ is_const e) ∧ (¬is_d_none_in d ⇒ is_e_lval e))
+show that P ==> not Q
+**************************)
+
+val lemma_dc1a =
+prove(`` ! d e.(is_d_none_in d ∧ ¬is_const e)
+	     ==> ~((is_d_none_in d ⇒ is_const e) ∧ (¬is_d_none_in d ⇒ is_e_lval e)) ``,
+NTAC 3 STRIP_TAC >>
+SIMP_TAC std_ss [] >>
+DISJ1_TAC>>
+METIS_TAC[]
+);
+
+
+val lemma_dc1b =
+prove(``
+(∀y. (λ(d,e). is_d_none_in (d) ∧ ¬is_const (e)) y ⇒
+             ($¬ ∘
+              (λ(d,e).
+                   (is_d_none_in (d) ⇒ is_const (e)) ∧
+                   (¬is_d_none_in (d) ⇒ is_e_lval (e)))) y)``,
+
+STRIP_TAC>>
+Cases_on `y`>>
+FULL_SIMP_TAC std_ss [lemma_dc1a] 
+);
+
+
+
+val lemma_dc1c =
+prove(`` ! d e. ((is_d_none_in d ⇒ is_const e) ∧ (¬is_d_none_in d ⇒ is_e_lval e))
+                     ==> ~(is_d_none_in d ∧ ¬is_const e) ``,
+NTAC 3 STRIP_TAC >>
+SIMP_TAC std_ss [] >>
+METIS_TAC[]
+);
+
+
+(***************************
+Show that
+INDEX_FIND 0 P l = SOME x ==> P(x)
+
+****************************)
+val lemma_dc2 =
+prove(``!l n. ((INDEX_FIND n (λ(d,e). is_d_none_in d ∧ ¬is_const e)
+                  l) = SOME x)  ==> (λ(d,e). is_d_none_in d ∧ ¬is_const e) (SND x) ``,
+Induct >| [
+FULL_SIMP_TAC list_ss [INDEX_FIND_def]
 ,
-NTAC 2 (
-RW.ONCE_RW_TAC[e_red_cases] >>
-EVAL_TAC>>
-FULL_SIMP_TAC std_ss [FUPDATE_EQ])
+REPEAT STRIP_TAC >>
+FULL_SIMP_TAC list_ss [INDEX_FIND_def]>>
+Cases_on `(λ(d,e). is_d_none_in d ∧ ¬is_const e) h` >>
+RW_TAC (list_ss) [] >>
+Q.PAT_X_ASSUM `∀n. _`
+( STRIP_ASSUME_TAC o (Q.SPECL [`SUC n`])) >>
+FULL_SIMP_TAC list_ss [INDEX_FIND_def]>>
+RW_TAC (list_ss) [] 
 ]
 );
 
 
-val prog_acc_s1a = ``e_acc (e_v (v_struct (^struct1))) (e_var("IPv4_h"))  ``;
-val prog_acc_s1b = ``e_v  (v_header (T) (^header1) ) ``;
-val stacks_s1    = ``(stacks_tup ^scopelist_s1 [])``;
+(***************************
+Show that 
+(INDEX_FIND n P l = NONE) = ~ EXISTS P l
 
+****************************)
 
-val test_acc_h1 =
-prove(`` (e_red  (^ctx_empty)(^prog_acc_s1a) 
-                  (^stacks_s1) ^R
-                  (^prog_acc_s1b) 
-                  (^stacks_s1) ^R)
-``,
-RW.ONCE_RW_TAC[e_red_cases] >>
-NTAC 2 (EVAL_TAC>>
-FULL_SIMP_TAC std_ss [])
+val lemma_dc3 =
+prove(``! l n. (( INDEX_FIND n (λ(d,e). is_d_none_in d ∧ ¬is_const e) l) = NONE) =
+       ~(EXISTS (λ(d,e). is_d_none_in d ∧ ¬is_const e) l)``,
+Induct >|[
+FULL_SIMP_TAC list_ss [INDEX_FIND_def]
+,
+FULL_SIMP_TAC list_ss [INDEX_FIND_def]>>
+Cases_on `(λ(d,e). is_d_none_in d ∧ ¬is_const e) h` >|[
+FULL_SIMP_TAC list_ss [SND]
+,
+FULL_SIMP_TAC list_ss [INDEX_FIND_def]
+]
+]
 );
+
+
+(***************************
+Show that for a generic P (Lemma T4)
+(INDEX_FIND n P l = NONE) = ~ EXISTS P
+****************************)
+
+val lemma_dc4 =
+prove(``!  (l: (d#e) list) n P. (( INDEX_FIND n P l) = NONE) = ~(EXISTS (P) l)``,
+Induct >|[
+FULL_SIMP_TAC list_ss [INDEX_FIND_def]
+,
+FULL_SIMP_TAC list_ss [INDEX_FIND_def]>>
+REPEAT STRIP_TAC >>
+Cases_on `P h` >>
+FULL_SIMP_TAC list_ss []
+]
+);
+
+
+
+
+
+
+(***************************
+Show that (equivelnt to above)
+(INDEX_FIND n P l = NONE) = EVERY ~P l
+Here just write P and substitute later.
+****************************)
+
+val lemma_dc5 =
+prove(``! l P n. (( INDEX_FIND n (P: (d#e -> bool)) l) = NONE) = (EVERY ($¬ ∘ P) l)``,
+FULL_SIMP_TAC list_ss [NOT_EXISTS, lemma_dc4]
+);
+
+
+
+(***************************
+WE CANT SHOW THIS:
+! l P n. (( INDEX_FIND n P l) = NONE) = ~(( INDEX_FIND n P l) = SOME x)
+BUT WE CAN SHOW
+! l P n. (( INDEX_FIND n P l) = NONE) ==> ~(( INDEX_FIND n P l) = SOME x)
+Here just write P and substitute later.
+****************************)
+
+val lemma_dc6a =
+prove(``! l P n. (( INDEX_FIND n P l) = NONE) ==> ~(( INDEX_FIND n P l) = SOME x) ``,
+FULL_SIMP_TAC (std_ss++optionSimps.OPTION_ss) [NOT_SOME_NONE, option_CLAUSES]
+);
+
+
+val lemma_dc6b =
+prove(``! l P n. (( INDEX_FIND n P l) = SOME x) ==> ~(( INDEX_FIND n P l) = NONE) ``,
+FULL_SIMP_TAC (std_ss++optionSimps.OPTION_ss) [NOT_SOME_NONE, option_CLAUSES]
+);
+
+(***************************
+Show that Lemma T6
+(?x . INDEX_FIND n P l = SOME x) = EXISTS P l
+Here just write P and substitute later.
+****************************)
+
+val lemma_dc7a =
+prove(``
+∀ (l: (d#e) list) n P. ~ (INDEX_FIND n P l = NONE) ⇔ EXISTS P l ``,
+REPEAT GEN_TAC >>
+ASSUME_TAC lemma_dc4>>
+Q.PAT_X_ASSUM `∀l n P. _`
+( STRIP_ASSUME_TAC o (Q.SPECL [`l`, `n`, `P`])) >>
+FULL_SIMP_TAC (std_ss) [combinTheory.o_DEF]
+);
+
+
+
+val lemma_dc7b =
+prove(``
+∀ (l: (d#e) list) n P.~ (INDEX_FIND n P l = NONE) = ? x. ( INDEX_FIND n P l) = SOME x``,
+REPEAT GEN_TAC >>
+Cases_on `INDEX_FIND n P l ` >>
+FULL_SIMP_TAC (std_ss) [NOT_SOME_NONE,option_CLAUSES ]
+);
+
+
+
+(*This is the ONE!!!!*)
+
+val lemma_dc7c =
+prove(``!  (l: (d#e) list) P n. (?x .(( INDEX_FIND n P l) = SOME x)) = (EXISTS P l)``,
+REPEAT GEN_TAC >>
+ASSUME_TAC lemma_dc4>>
+Q.PAT_X_ASSUM `∀l n P. _`
+( STRIP_ASSUME_TAC o (Q.SPECL [`l`, `n`, `P`])) >>
+ASSUME_TAC lemma_dc7a >>
+Q.PAT_X_ASSUM `∀l n P. _`
+( STRIP_ASSUME_TAC o (Q.SPECL [`l`, `n`, `P`])) >>
+ASSUME_TAC lemma_dc7b>>
+Q.PAT_X_ASSUM `∀l n P. _`
+( STRIP_ASSUME_TAC o (Q.SPECL [`l`, `n`, `P`])) >>
+
+FULL_SIMP_TAC (srw_ss()) [lemma_dc7b, lemma_dc7a , lemma_dc4 ]
+);
+
+
+
+
+
+(***************************
+Show Lemma T2.1
+! PQ . (∀x. P x ⇒ Q x) ⇒ (∃x. FI n P x) ⇒ ∃x. FI n Q x
+****************************)
+
+
+val lemma_dc_mono1 =
+prove (``! P Q l. ((! (x) . (P x ==>  Q x) ) ==>
+((EXISTS P l) ==>
+(EXISTS Q l)))``,
+REPEAT STRIP_TAC >>
+ASSUME_TAC MONO_EXISTS >>
+FULL_SIMP_TAC list_ss[MONO_EXISTS ]
+);
+
+val lemma_dc_mono2 =
+prove (``
+! P Q l n. ((!  (y : (d#e)) . (P y ==>  Q y) ) ==>
+((? v. INDEX_FIND n P l = SOME v) ==>
+(? v. INDEX_FIND n Q l = SOME v)))
+
+``,
+REPEAT STRIP_TAC >>
+ASSUME_TAC (ISPECL [``P:(d # e) -> bool``, ``Q:(d # e) -> bool``, ``l:(d # e) list``] lemma_dc_mono1) >>
+(*twice*)
+ASSUME_TAC  lemma_dc7c >>
+Q.PAT_X_ASSUM `∀l P n. (∃x. INDEX_FIND n P l = SOME x) ⇔ EXISTS P l`
+( STRIP_ASSUME_TAC o (Q.SPECL [`l`, `P`, `n`])) >>
+
+ASSUME_TAC  lemma_dc7c >>
+Q.PAT_X_ASSUM `∀l P n. (∃x. INDEX_FIND n P l = SOME x) ⇔ EXISTS P l`
+( STRIP_ASSUME_TAC o (Q.SPECL [`l`, `Q`, `n`])) >>
+RES_TAC>>
+fs []
+);
+
+
+
+
+
+(***************************
+The Big lemma
+****************************)
+
+val lemma_args1 =
+prove (`` ! dl el i. (unred_arg_index dl el = SOME i) ==> ~ check_args_red dl el ``,
+Cases_on `dl`>>
+Cases_on `el` >|[
+RW_TAC (srw_ss()) [unred_arg_index_def]>>
+RW_TAC (srw_ss()) [check_args_red_def]>>
+Cases_on ` find_unred_arg [] []`>>
+FULL_SIMP_TAC (list_ss) [find_unred_arg_def] >>
+FULL_SIMP_TAC (list_ss) [INDEX_FIND_def] 
+
+,
+RW_TAC (srw_ss()) [unred_arg_index_def]>>
+RW_TAC (srw_ss()) [check_args_red_def]>>
+Cases_on ` find_unred_arg [] (h::t)`>>
+FULL_SIMP_TAC (list_ss) [find_unred_arg_def] >>
+FULL_SIMP_TAC (list_ss) [INDEX_FIND_def, ZIP_def] 
+,
+RW_TAC (srw_ss()) [unred_arg_index_def]>>
+RW_TAC (srw_ss()) [check_args_red_def]>>
+Cases_on ` find_unred_arg (h::t) []`>>
+FULL_SIMP_TAC (list_ss) [find_unred_arg_def] >>
+FULL_SIMP_TAC (list_ss) [INDEX_FIND_def, ZIP_def] 
+,
+
+
+SIMP_TAC (list_ss) [unred_arg_index_def]>>
+REWRITE_TAC [check_args_red_def]>>
+Cases_on ` find_unred_arg (h::t) (h'::t')`
+>|[
+REPEAT STRIP_TAC >>
+FULL_SIMP_TAC (list_ss) [find_unred_arg_def] >>
+FULL_SIMP_TAC (list_ss) [INDEX_FIND_def, ZIP_def]
+,
+
+FULL_SIMP_TAC (list_ss) [find_unred_arg_def] >>
+FULL_SIMP_TAC (list_ss) [INDEX_FIND_def, ZIP_def]>>
+
+Cases_on `(is_d_none_in h ∧ ¬is_const h')` >| [
+FULL_SIMP_TAC (list_ss) [is_arg_red_def]
+,
+STRIP_TAC >>
+FULL_SIMP_TAC (list_ss) [find_unred_arg_def] >>
+FULL_SIMP_TAC (list_ss) [INDEX_FIND_def, ZIP_def]>>
+FULL_SIMP_TAC (list_ss) [is_arg_red_def]>>
+STRIP_TAC >>
+DISJ2_TAC>>
+ASSUME_TAC lemma_dc_mono2 >>
+Q.PAT_X_ASSUM `∀P Q l n. _`
+( STRIP_ASSUME_TAC o (Q.SPECL [
+`(λ(d,e). is_d_none_in d ∧ ¬is_const e) `,
+`$¬ ∘ (λ(d,e). ((is_d_none_in d ⇒ is_const e) ∧
+                (¬is_d_none_in d ⇒ is_e_lval e)))`,
+`ZIP (t,t')`,
+`1`
+])) >>
+FULL_SIMP_TAC std_ss [lemma_dc1b] >>
+
+RES_TAC>>
+ASSUME_TAC lemma_dc7c>>
+
+Q.PAT_X_ASSUM `∀l P n. _`
+( STRIP_ASSUME_TAC o (Q.SPECL [
+`ZIP (t,t') `,
+`$¬ ∘ (λ(d,e). ((is_d_none_in d ⇒ is_const e) ∧
+                (¬is_d_none_in d ⇒ is_e_lval e)))`,
+`1`
+])) >>
+fs[]
+
+]]]);
+
+(*******************************************)
+
+
+fun OPEN_EXP_RED_TAC exp_term =
+(Q.PAT_X_ASSUM `e_red c scope scopest ^exp_term exp2 fr` (fn thm => ASSUME_TAC (SIMP_RULE (srw_ss()) [Once e_red_cases] thm)))
+
+
+
+val same_frame_exp_def = Define `
+ same_frame_exp (frame:Frame_list) frame' (e:e) e'  =
+((frame = frame') /\ (e = e'))
+`;
+
+
+val lemma_v_red_forall =
+prove(`` ! c s sl e l fl.
+~ e_red c s sl (e_v (l)) e fl   ``,
+RW_TAC (srw_ss()) [Once e_red_cases]
+);
+
+
+
+val det_exp_def = Define `
+ det_exp e = ! c scope scopest e' e'' frame frame'.
+(e_red c scope scopest e e' frame )
+/\
+(e_red c scope scopest e e'' frame' ) 
+==>
+(same_frame_exp frame frame' e' e'')
+`;
+
+
+val det_exp_list_def = Define `
+   det_exp_list (l : e list)  = !(x : e). MEM x l ==> det_exp(x)
+`;
+
+(*Replace the one that in p4_exec_semTheory once fixed*)
+Theorem unred_arg_index_in_range:
+ !d_l e_l i. unred_arg_index d_l e_l = SOME i ==> i < LENGTH e_l
+Proof
+cheat
+QED
+
+
+
+val P4EXP_det =
+prove (
+``
+(!e. det_exp e) /\
+(! l: e list. det_exp_list l)
+``,
+Induct >| [
+RW_TAC (srw_ss()) [same_frame_exp_def, det_exp_def, Once e_red_cases]
+,
+RW_TAC (srw_ss()) [det_exp_def] >>
+FULL_SIMP_TAC (srw_ss()) [det_exp_def, Once e_red_cases, same_frame_exp_def]
+,
+RW_TAC (srw_ss()) [det_exp_def] >>
+FULL_SIMP_TAC (srw_ss()) [det_exp_def, Once e_red_cases, same_frame_exp_def]
+,
+RW_TAC (srw_ss()) [det_exp_def] >>
+FULL_SIMP_TAC (srw_ss()) [Once e_red_cases, same_frame_exp_def]
+,
+
+NTAC 2 (
+SIMP_TAC (srw_ss()) [det_exp_def] >>
+REPEAT STRIP_TAC >>
+OPEN_EXP_RED_TAC ``e_acc e e'`` >>
+REV_FULL_SIMP_TAC (srw_ss()) [] >>
+RW_TAC (srw_ss()) []) >>
+TRY (OPEN_EXP_RED_TAC ``(e_acc (e_v (_)) (e_v (_)))`` ) >>
+RW_TAC (srw_ss()) [] >>
+FULL_SIMP_TAC (srw_ss()) [det_exp_def,lemma_v_red_forall, same_frame_exp_def] >>
+RES_TAC 
+,
+
+SIMP_TAC (srw_ss()) [det_exp_def] >>
+REPEAT STRIP_TAC >>
+OPEN_EXP_RED_TAC ``(e_unop u e)`` >>
+REV_FULL_SIMP_TAC (srw_ss()) [] >>
+RW_TAC (srw_ss()) [] >>
+
+OPEN_EXP_RED_TAC ``(e_unop u e)`` >>
+RW_TAC (srw_ss()) [] >>
+FULL_SIMP_TAC (srw_ss()) [det_exp_def] >>
+RES_TAC >>
+FULL_SIMP_TAC (srw_ss()) [same_frame_exp_def] >>
+REPEAT (IMP_RES_TAC lemma_v_red_forall >>
+FULL_SIMP_TAC (srw_ss()) [det_exp_def] )
+,
+(*****************************)
+(*    binop case             *)
+(*****************************)
+
+(
+SIMP_TAC (srw_ss()) [det_exp_def] >>
+REPEAT STRIP_TAC >>
+OPEN_EXP_RED_TAC ``(e_binop e b e')`` >>
+REV_FULL_SIMP_TAC (srw_ss()) [] >>
+RW_TAC (srw_ss()) [] 
+
+) >- (      (*e_binop e b e'*)
+
+OPEN_EXP_RED_TAC ``(e_binop e b e')`` >>
+RW_TAC (srw_ss()) [] >>
+IMP_RES_TAC lemma_v_red_forall >>
+FULL_SIMP_TAC (srw_ss()) [det_exp_def,lemma_v_red_forall, same_frame_exp_def] >>
+RES_TAC >>
+FULL_SIMP_TAC (srw_ss()) [Once same_frame_exp_def]
+) >-  (
+
+              (*e_binop (e_v v) b e'*)
+OPEN_EXP_RED_TAC ``(e_binop (e_v v) b e')`` >>
+RW_TAC (srw_ss()) []>>
+IMP_RES_TAC lemma_v_red_forall >>
+FULL_SIMP_TAC (srw_ss()) [det_exp_def] >>
+RES_TAC >>
+FULL_SIMP_TAC (srw_ss()) [Once same_frame_exp_def] ) >> (
+(*e_mul case and after, use those as much as needed.*)
+OPEN_EXP_RED_TAC ``(e_binop a b c)`` >>
+RW_TAC (srw_ss()) [] >>
+IMP_RES_TAC lemma_v_red_forall >>
+FULL_SIMP_TAC (srw_ss()) [det_exp_def,lemma_v_red_forall, same_frame_exp_def, option_case_def])
+
+
+,
+
+SIMP_TAC (srw_ss()) [det_exp_def] >>
+REPEAT STRIP_TAC >>
+OPEN_EXP_RED_TAC ``(e_concat e e')`` >>
+REV_FULL_SIMP_TAC (srw_ss()) [] >>
+RW_TAC (srw_ss()) []
+
+,
+
+SIMP_TAC (srw_ss()) [det_exp_def] >>
+REPEAT STRIP_TAC >>
+OPEN_EXP_RED_TAC ``(e_slice e e' e'')`` >>
+REV_FULL_SIMP_TAC (srw_ss()) [] >>
+RW_TAC (srw_ss()) []
+
+,
+
+
+(*****************************)
+(*    e_func_call            *)
+(*****************************)
+SIMP_TAC (srw_ss()) [det_exp_def] >>
+REPEAT STRIP_TAC >>
+OPEN_EXP_RED_TAC ``(e_func_call s l)`` >>
+REV_FULL_SIMP_TAC (srw_ss()) [] >>
+RW_TAC (srw_ss()) []  >| [
+
+(*first subgoal*)
+OPEN_EXP_RED_TAC ``(e_func_call s l)`` >>
+RW_TAC (srw_ss()) [] >| [
+
+REV_FULL_SIMP_TAC (list_ss) [rich_listTheory.MAP_FST_funs, same_frame_exp_def] >>
+IMP_RES_TAC lemma_MAP4>>
+METIS_TAC []
+,
+REV_FULL_SIMP_TAC (srw_ss()) [same_frame_exp_def] >>
+IMP_RES_TAC lemma_MAP5>>
+RES_TAC >>	
+IMP_RES_TAC lemma_args1 >>
+METIS_TAC[]]
+,
+(*second subgoal*)
+OPEN_EXP_RED_TAC ``(e_func_call s l)`` >>
+RW_TAC (srw_ss()) [] >|[
+
+REV_FULL_SIMP_TAC (srw_ss()) [same_frame_exp_def] >>
+ASSUME_TAC lemma_MAP5>>
+PAT_ASSUM `` ∀l l'. _ ``
+( STRIP_ASSUME_TAC o (Q.SPECL [`e_x_d_list`,`e_e'_x_d_list` ])) >> 
+IMP_RES_TAC lemma_args1 >>
+METIS_TAC[]
+,
+(**first show that the d is the same in both lists, thus the i = i'*)
+REV_FULL_SIMP_TAC (srw_ss()) [] >>
+IMP_RES_TAC lemma_MAP6 >>
+`i = i'` by METIS_TAC [ option_case_def]>>
+
+(*Now try to show that the EL i l is deterministic*)
+REV_FULL_SIMP_TAC (srw_ss()) [same_frame_exp_def, det_exp_list_def] >>
+PAT_ASSUM `` ∀x._``
+( STRIP_ASSUME_TAC o (Q.SPECL [`(EL i (MAP (λ(e_,e'_,x_,d_). e_) (e_e'_x_d_list:(e#e#string#d)list)))` ])) >>
+IMP_RES_TAC unred_arg_index_in_range  >>
+IMP_RES_TAC EL_MEM >>
+FULL_SIMP_TAC list_ss [det_exp_def]  >>
+RES_TAC >>
+FULL_SIMP_TAC list_ss [same_frame_exp_def]>>
+rw[] >> rw[]
+]
+]
+
+,
+
+(*****************************)
+(*   e_select                *)
+(*****************************)
+
+SIMP_TAC (srw_ss()) [det_exp_def] >>
+REPEAT STRIP_TAC >>
+OPEN_EXP_RED_TAC ``(e_select e l s)`` >>
+REV_FULL_SIMP_TAC (srw_ss()) [] >>
+
+(*first + second + beginning of third subgoal*)
+ (OPEN_EXP_RED_TAC ``(e_select e l s)`` >>
+REV_FULL_SIMP_TAC (srw_ss()) [] >>
+FULL_SIMP_TAC (srw_ss()) [same_frame_exp_def] >>
+IMP_RES_TAC lemma_v_red_forall) >>
+FULL_SIMP_TAC (srw_ss()) [det_exp_def]>>
+RES_TAC>>
+FULL_SIMP_TAC (srw_ss()) [Once same_frame_exp_def ] 
+
+,
+
+FULL_SIMP_TAC list_ss [det_exp_list_def]
+,
+
+FULL_SIMP_TAC list_ss [det_exp_list_def] >>
+REPEAT STRIP_TAC >>
+rw []
+
+]
+);
+
+
+
+
+(******** SAME SATE and STMT DEF ************)
+val same_state_stmt_def = Define `
+ same_state_stmt (st:state) st'  =
+((st = st'))
+`;
+
+
+val det_stmt_def = Define `
+ det_stmt stm = ! (c:ctx) (ss:scopes_stack) (s':state) (s'':state) (Gscope:Gscope) (f:string) status.
+(stmt_red c (state_P4 Gscope  ([(f,stm,ss)])  status) (s'))
+/\
+(stmt_red c (state_P4 Gscope  ([(f,stm,ss)])  status) (s''))
+==>
+( same_state_stmt s' s'')
+`;
+
+
+
+
+fun OPEN_STMT_RED_TAC stm_term =
+(Q.PAT_X_ASSUM `stmt_red c (state_P4 Gs [(f,^stm_term ,ss)] st) state` (fn thm => ASSUME_TAC (SIMP_RULE (srw_ss()) [Once stmt_red_cases] thm)))
+
+
+
+
+
+
+val P4Sem_det =
+prove (
+``
+(!stm. det_stmt stm) 
+``
+
+Induct >|[
+RW_TAC (srw_ss()) [det_stmt_def] >>
+OPEN_STMT_RED_TAC ``stmt_empty`` >>
+fs []
+,
+
+
+SIMP_TAC (srw_ss()) [det_stmt_def] >>
+REPEAT STRIP_TAC >>
+OPEN_STMT_RED_TAC ``(stmt_ass l e)`` >>
+REV_FULL_SIMP_TAC (srw_ss()) [] >>
+
+(*first + second subgoal*)
+OPEN_STMT_RED_TAC ``(stmt_ass l e)`` >>
+REV_FULL_SIMP_TAC (srw_ss()) [] >>
+RW_TAC (srw_ss()) []>>
+REV_FULL_SIMP_TAC (srw_ss())  [assign_def, same_state_stmt_def] >>
+IMP_RES_TAC lemma_v_red_forall>|[
+METIS_TAC [ option_case_def]
+,
+ASSUME_TAC P4EXP_det >>
+fs [det_exp_def]  >>
+RES_TAC >>
+fs [same_frame_exp_def]
+]
+
+,
+
+(*****************************)
+(*   stmt_cond                *)
+(*****************************)
+
+SIMP_TAC (srw_ss()) [det_stmt_def] >>
+REPEAT STRIP_TAC >>
+OPEN_STMT_RED_TAC ``stmt_cond e stm stm'`` >>
+REV_FULL_SIMP_TAC (srw_ss()) [] >>
+
+(*first subgoal*)
+OPEN_STMT_RED_TAC ``stmt_cond e stm stm'`` >>
+REV_FULL_SIMP_TAC (srw_ss()) [] >>
+FULL_SIMP_TAC (srw_ss()) [Once same_state_stmt_def]>>
+IMP_RES_TAC lemma_v_red_forall>>
+FULL_SIMP_TAC (srw_ss()) [det_stmt_def,lemma_v_red_forall] >>
+
+ASSUME_TAC P4EXP_det >>
+fs [det_exp_def]  >>
+RES_TAC >>
+fs [same_frame_exp_def]
+
+,
+
+(*****************************)
+(*   stmt_declare            *)
+(*****************************)
+NTAC 2 (SIMP_TAC (srw_ss()) [det_stmt_def] >>
+REPEAT STRIP_TAC >>
+OPEN_STMT_RED_TAC ``stmt_declare s t`` >>
+REV_FULL_SIMP_TAC (srw_ss()) []) >> 
+FULL_SIMP_TAC (srw_ss()) [Once same_state_stmt_def]
+,
+
+(*****************************)
+(*   stmt_block              *)
+(*****************************)
+NTAC 2 (SIMP_TAC (srw_ss()) [det_stmt_def] >>
+REPEAT STRIP_TAC >>
+OPEN_STMT_RED_TAC ``stmt_block stm`` >>
+REV_FULL_SIMP_TAC (srw_ss()) []) >> 
+FULL_SIMP_TAC (srw_ss()) [Once same_state_stmt_def]
+
+,
+
+(*****************************)
+(*   stmt_ip                 *)
+(*****************************)
+(NTAC 2 (SIMP_TAC (srw_ss()) [det_stmt_def] >>
+REPEAT STRIP_TAC >>
+OPEN_STMT_RED_TAC ``stmt_block_ip stm`` >>
+REV_FULL_SIMP_TAC (srw_ss()) []) >> 
+FULL_SIMP_TAC (srw_ss()) [Once same_state_stmt_def]) >- (
+FULL_SIMP_TAC (srw_ss()) [det_stmt_def] >>
+RES_TAC >>
+FULL_SIMP_TAC (srw_ss()) [Once same_state_stmt_def] ) >>
+OPEN_STMT_RED_TAC ``stmt_empty`` >>
+REV_FULL_SIMP_TAC (srw_ss()) []
+,
+(*****************************)
+(*   stmt_ret                *)
+(*****************************)
+(NTAC 2 ( SIMP_TAC (srw_ss()) [det_stmt_def] >>
+REPEAT STRIP_TAC >>
+OPEN_STMT_RED_TAC ``(stmt_ret e)`` >>
+REV_FULL_SIMP_TAC (srw_ss()) [] ) >> 
+FULL_SIMP_TAC (srw_ss()) [Once same_state_stmt_def]) >>
+
+FULL_SIMP_TAC (srw_ss()) [det_exp_def] >>
+RES_TAC >>
+FULL_SIMP_TAC (srw_ss()) [Once same_state_stmt_def] >>
+IMP_RES_TAC lemma_v_red_forall>>
+
+ASSUME_TAC P4EXP_det >>
+fs [det_exp_def]  >>
+RES_TAC >>
+fs [same_frame_exp_def]
+,
+
+(*****************************)
+(*   stmt_seq                *)
+(*****************************)
+
+(NTAC 2 (SIMP_TAC (srw_ss()) [det_stmt_def] >>
+REPEAT STRIP_TAC >>
+OPEN_STMT_RED_TAC ``(stmt_seq stm stm')`` >>
+REV_FULL_SIMP_TAC (srw_ss()) []) >> 
+FULL_SIMP_TAC (srw_ss()) [Once same_state_stmt_def]) >>
+FULL_SIMP_TAC (srw_ss()) [det_stmt_def] >>
+RES_TAC >>
+FULL_SIMP_TAC (srw_ss()) [Once same_state_stmt_def, Once same_frame_exp_def ] >>
+OPEN_STMT_RED_TAC ``stmt_empty`` >>
+REV_FULL_SIMP_TAC (srw_ss()) []
+
+
+,
+
+(*****************************)
+(*   stmt_verify             *)
+(*****************************)
+(NTAC 2 (SIMP_TAC (srw_ss()) [det_stmt_def] >>
+REPEAT STRIP_TAC >>
+OPEN_STMT_RED_TAC ``(stmt_verify e e')`` >>
+REV_FULL_SIMP_TAC (srw_ss()) []) >> 
+FULL_SIMP_TAC (srw_ss()) [Once same_state_stmt_def]) >>
+IMP_RES_TAC lemma_v_red_forall>>
+FULL_SIMP_TAC (srw_ss()) [det_exp_def,lemma_v_red_forall] >>
+RES_TAC>>
+FULL_SIMP_TAC (srw_ss()) [Once same_frame_exp_def]>>
+ASSUME_TAC P4EXP_det >>
+fs [det_exp_def]  >>
+RES_TAC >>
+fs [same_frame_exp_def]
+
+,
+
+
+(*****************************)
+(*   stmt_trans              *)
+(*****************************)
+(NTAC 2 (SIMP_TAC (srw_ss()) [det_stmt_def] >>
+REPEAT STRIP_TAC >>
+OPEN_STMT_RED_TAC ``(stmt_trans e)`` >>
+REV_FULL_SIMP_TAC (srw_ss()) []) >> 
+FULL_SIMP_TAC (srw_ss()) [Once same_state_stmt_def]) >>
+IMP_RES_TAC lemma_v_red_forall>>
+FULL_SIMP_TAC (srw_ss()) [det_exp_def,lemma_v_red_forall] >>
+RES_TAC>>
+FULL_SIMP_TAC (srw_ss()) [Once same_frame_exp_def] >>
+ASSUME_TAC P4EXP_det >>
+fs [det_exp_def]  >>
+RES_TAC >>
+fs [same_frame_exp_def]
+
+,
+
+(*****************************)
+(*   stmt_app                *)
+(*****************************)
+(NTAC 2 (SIMP_TAC (srw_ss()) [det_stmt_def] >>
+REPEAT STRIP_TAC >>
+OPEN_STMT_RED_TAC `` (stmt_app s e)`` >>
+REV_FULL_SIMP_TAC (srw_ss()) []) >> 
+FULL_SIMP_TAC (srw_ss()) [Once same_state_stmt_def]) >>
+IMP_RES_TAC lemma_v_red_forall>>
+FULL_SIMP_TAC (srw_ss()) [det_exp_def,lemma_v_red_forall] >>
+RES_TAC >>
+FULL_SIMP_TAC (srw_ss()) [Once same_frame_exp_def]>>
+ASSUME_TAC P4EXP_det >>
+fs [det_exp_def]  >>
+RES_TAC >>
+fs [same_frame_exp_def]
+
+,
+
+(NTAC 2 (SIMP_TAC (srw_ss()) [det_stmt_def] >>
+REPEAT STRIP_TAC >>
+OPEN_STMT_RED_TAC ``(stmt_ext_sem)`` >>
+REV_FULL_SIMP_TAC (srw_ss()) []) >> 
+FULL_SIMP_TAC (srw_ss()) [Once same_state_stmt_def] ) >>
+REV_FULL_SIMP_TAC (srw_ss()) [] >>
+
+???
+]);
 
